Proved that the new semantics is deterministic, i.e. the final result is independent of garbage collection. Cleanup in progress.

theories/L6_PCPS/space_sem.v
@@ -3,15 +3,20 @@
  *)
 
 From Coq Require Import NArith.BinNat Relations.Relations MSets.MSets
-     MSets.MSetRBT Lists.List omega.Omega Sets.Ensembles Relations.Relations.
+         MSets.MSetRBT Lists.List omega.Omega Sets.Ensembles Relations.Relations
+         Classes.Morphisms.
 From ExtLib Require Import Structures.Monad Data.Monads.OptionMonad Core.Type.
-From L6 Require Import cps eval List_util Ensembles_util functions identifiers.
+From L6 Require Import cps cps_util eval List_util Ensembles_util functions
+        identifiers.
+From Libraries Require Import Coqlib.
 
 
 Module Type Heap.
 
   Parameter loc : Type.
-  
+
+  Parameter loc_dec : forall (l1 l2 : loc), { l1 = l2 } + { l1 <> l2 }.
+
   Parameter heap : Type -> Type. 
   
   Parameter emp : forall {A}, heap A.
@@ -40,7 +45,7 @@ Module Type Heap.
     forall A (x : A) (l1 l2 : loc) (H H' : heap A),
       l1 <> l2 ->
       alloc x H = (l1, H') ->
-      get l2 H' = get l1 H'. 
+      get l2 H' = get l2 H. 
 
   Parameter alloc_fresh :
     forall A (x : A) (l : loc) (H H' : heap A),
@@ -79,7 +84,7 @@ Module Type Heap.
     forall {A} (H1 H2 H : heap A) (l : loc) (v : A),
       splits H H1 H2 ->
       get l H = Some v ->
-      (get l H1 = Some v /\ get l H2 = None) /\
+      (get l H1 = Some v /\ get l H2 = None) \/
       (get l H2 = None /\ get l H2 = Some v).
 
   Parameter splits_spec_None :
@@ -87,74 +92,264 @@ Module Type Heap.
       splits H H1 H2 ->
       get l H = None ->
       get l H1 = None /\ get l H2 = None.
+    
+  Definition subheap {A} (H1 H2 : heap A) :=
+    forall x v, get x H1 = Some v -> get x H2 = Some v. 
 
+  Infix "⊑" := subheap (at level 70, no associativity).
+
+  Lemma splits_subheap_l {A} (H H1 H2 : heap A) : 
+    splits H H1 H2 -> H1 ⊑ H.
+  Proof.
+    intros Hs l v Hget. destruct (get l H) eqn:Heq'.
+    - eapply splits_spec_Some in Heq'; eauto.
+      destruct Heq' as [[Heq1 Heq22] | [Heq1 Heq2]]; congruence.
+    -  eapply splits_spec_None in Heq'; eauto.
+       destruct Heq'; congruence.
+  Qed.
+
+  Lemma splits_subheap_r {A} (H H1 H2 : heap A) : 
+    splits H H1 H2 -> H2 ⊑ H.
+  Proof.
+    intros Hs l v Hget. destruct (get l H) eqn:Heq'.
+    - eapply splits_spec_Some in Heq'; eauto.
+      destruct Heq' as [[Heq1 Heq22] | [Heq1 Heq2]]; congruence.
+    -  eapply splits_spec_None in Heq'; eauto.
+       destruct Heq'; congruence.
+  Qed.
+
+  Definition heap_eq {A} (S : Ensemble loc) (H1 H2 : heap A) :=
+    forall x, x \in S -> get x H1 = get x H2.
+
+  Notation  "S |- H1 ≡ H2" := (heap_eq S H1 H2) (at level 70, no associativity).
+
+  Instance Equivalence_heap_eq {A} S : Equivalence (@heap_eq A S).
+  Proof.
+    constructor. now firstorder. now firstorder.
+    intros x y z H1 H2 l Hin. rewrite H1; firstorder.
+  Qed.
+
+  Instance Proper_heap_eq {A} : Proper (Same_set loc ==> eq ==> eq ==> iff) (@heap_eq A).
+  Proof.
+    intros S1 S2 Heq x1 x2 Heq1 y1 y2 Heq2; subst. firstorder.
+  Qed.
+
+  Lemma alloc_subheap {A} (H1 H1' : heap A) l v :
+    alloc v H1 = (l, H1') ->
+    H1 ⊑ H1'.
+  Proof.
+    intros Ha x v' Hget. destruct (loc_dec x l); subst.
+    + erewrite alloc_fresh in Hget; eauto; congruence.
+    + erewrite gao; eauto.
+  Qed.
+
+  Definition dom {A} (H : heap A) : Ensemble loc :=
+    domain (fun l => get l H).
+   
+  Lemma dom_subheap {A} (H1 H2 : heap A) :
+    H1 ⊑ H2 ->
+    dom H1 \subset dom H2. 
+  Proof.
+    firstorder.
+  Qed.
+
+  Lemma heap_eq_antimon {A} S1 S2 (H1 H2 : heap A) :
+    S1 \subset S2 ->
+    S2 |- H1 ≡ H2 ->
+    S1 |- H1 ≡ H2.
+  Proof.
+    firstorder.
+  Qed.
+  
 End Heap.
 
 Module Sem (H : Heap).
 
   Import H.
 
+  (** * Heap definitions *)
+
   (* All the values are boxed *)
   Definition env := M.t loc.
-  
+
+  (** The type of heap values *)
   Inductive val : Type :=
   | Vconstr: cTag -> list loc -> val
   | Vfun: env -> fundefs -> val.
-
+  
   (** The result of the evaluation *)
   Definition res := (loc * heap val)%type.
 
-  (** Equivalence of results *)
-  Inductive res_equiv : res -> res -> Prop :=
-  | Vconstr_eq :
-      forall l1 l2 H1 H2 c1 ls1 c2 ls2,
-        get l1 H1 = Some (Vconstr c1 ls1) ->
-        get l1 H1 = Some (Vconstr c2 ls2) ->
-        Forall2 (fun l1 l2 => res_equiv (l1, H1) (l2, H2)) ls1 ls2 ->
-        res_equiv (l1, H1) (l2, H2)
-  | Vfun_eq :
-      forall l1 l2 H1 H2 rho1 rho2 B,
-        get l1 H1 = Some (Vfun rho1 B) ->
-        get l1 H1 = Some (Vfun rho2 B) ->
-        (forall x,  x \in (occurs_free_fundefs B) ->
-               (exists l1 l2, M.get x rho1 = Some l1 /\
-                        M.get x rho2 = Some l2 /\
-                        res_equiv (l1, H1) (l2, H2)) \/
-               (M.get x rho1 = None /\ M.get x rho2 = None)) ->
-        res_equiv (l1, H1) (l2, H2).
+  (** Approximation of results with fuel *)
+  Fixpoint res_approx_fuel (n : nat) (r1 r2 : res) : Prop :=
+    let (l1, H1) := r1 in
+    let (l2, H2) := r2 in     
+    forall v1,
+      get l1 H1 = Some v1->
+      exists v2,
+        get l2 H2 = Some v2 /\
+        match v1, v2 with
+          | Vconstr c1 ls1, Vconstr c2 ls2 =>
+            c1 = c2 /\
+            forall i, (i < n)%nat ->
+                 match n with
+                   | 0%nat => True
+                   | S n' =>
+                     Forall2
+                       (fun l1 l2 => res_approx_fuel (n'-(n'-i)) (l1, H1) (l2, H2)) ls1 ls2
+                 end
+          | Vfun rho1 B1, Vfun rho2 B2 =>
+            B1 = B2 /\
+            (forall i, (i < n)%nat ->
+                  match n with
+                    | 0%nat => True
+                    | S n' =>
+                      forall x, x \in (occurs_free_fundefs B1) ->
+                                 (exists l1 l2, M.get x rho1 = Some l1 /\
+                                           M.get x rho2 = Some l2 /\
+                                           res_approx_fuel (n'-(n'-i)) (l1, H1) (l2, H2)) \/
+                                 (M.get x rho1 = None /\ M.get x rho2 = None)
+                  end)
+          | _, _ => False
+        end.
+
+  (** Equivalent definition, unfolding the recursion *)
+  Definition res_approx_fuel' (n : nat) (r1 r2 : res) : Prop :=
+    let (l1, H1) := r1 in
+    let (l2, H2) := r2 in
+    forall v1,
+      get l1 H1 = Some v1->
+      exists v2, get l2 H2 = Some v2 /\
+            match v1, v2 with
+              | Vconstr c1 ls1, Vconstr c2 ls2 =>
+                c1 = c2 /\
+                forall i, (i < n)%nat ->
+                     Forall2 (fun l1 l2 => res_approx_fuel i (l1, H1) (l2, H2)) ls1 ls2
+              | Vfun rho1 B1, Vfun rho2 B2 =>
+                B1 = B2 /\
+                forall i x, (i < n)%nat -> 
+                       x \in (occurs_free_fundefs B1) ->
+                             (exists l1 l2, M.get x rho1 = Some l1 /\
+                                       M.get x rho2 = Some l2 /\
+                                       res_approx_fuel i (l1, H1) (l2, H2)) \/
+                             (M.get x rho1 = None /\ M.get x rho2 = None)
+              | _, _ => False
+            end.
+  
+  (** Equivalence of the two definitions *)
+  Lemma res_approx_fuel_eq n r1 r2 :
+    res_approx_fuel n r1 r2 <-> res_approx_fuel' n r1 r2.
+  Proof.
+    destruct n; destruct r1 as [l1 H1]; destruct r2 as [l2 H2]; split; intros H v1 Hget1; 
+    destruct (H v1 Hget1) as [v2 [Hget2 H']]; destruct v1; destruct v2;
+    try (now intros; omega); try (destruct H' as [H1' H2']; repeat eexists; eauto; simpl; split; eauto; intros; omega).
+    - destruct H' as [H1' H2'].
+      repeat eexists; eauto; simpl; eauto; split; eauto; intros.
+      assert (Heq : (i = n - (n - i))%nat) by omega. rewrite Heq.
+      eauto.
+    - destruct H' as [H1' H2'].
+      repeat eexists; eauto; simpl; eauto; split; eauto; intros.
+      assert (Heq : (i = n - (n - i))%nat) by omega. rewrite Heq.
+      eauto.
+    - destruct H' as [H1' H2'].
+      repeat eexists; eauto; simpl; eauto; split; eauto; intros.
+      assert (Heq : (i = n - (n - i))%nat) by omega. rewrite <- Heq.
+      eauto.
+    - destruct H' as [H1' H2'].
+      repeat eexists; eauto; simpl; eauto; split; eauto; intros.
+      assert (Heq : (i = n - (n - i))%nat) by omega. rewrite <- Heq.
+      eauto.
+  Qed.
+
+  Opaque res_approx_fuel.
+
+  (** Result equivalence *)
+  Definition res_equiv (r1 r2 : res) : Prop :=
+    forall n, res_approx_fuel' n r1 r2 /\ res_approx_fuel' n r2 r1.
   
   Infix "≈" := res_equiv (at level 70, no associativity).
+  
+  (** Approximation lifted to the environments *)
+  Definition heap_env_approx (S : Ensemble var) p1 p2 : Prop :=
+    let '(H1, rho1) := p1 in
+    let '(H2, rho2) := p2 in
+    forall x l, x \in S ->
+           M.get x rho1 = Some l ->
+           exists l', M.get x rho2 = Some l' /\
+                 (l, H1) ≈ (l', H2).
+  
+  (** Equivalence lifted to the environments *)
+  Definition heap_env_equiv S p1 p2 : Prop :=
+    heap_env_approx S p1 p2 /\
+    heap_env_approx S p2 p1.
 
+  Notation "S |- p1 ⩪ p2" := (heap_env_equiv S p1 p2)
+                               (at level 70, no associativity).
 
-  (** The locations that appear on values *)
+  (** The image of the environment *)
+  Definition env_locs (rho : env) S := image' (fun x => M.get x rho) S.
+  
+  (** The locations that appear on a value *)
   Definition locs (v : val) : Ensemble loc :=
     match v with
       | Vconstr t ls => FromList ls
       | Vfun rho B =>
-        (* Take only the relevant part of the environment instead of its domain *)
-        image' (fun x => M.get x rho) (occurs_free_fundefs B)
+        (* Take only the relevant part of the environment instead
+           of its whole codomain *)
+        env_locs rho (occurs_free_fundefs B)
     end.
-  
-  Definition post (H : heap val) (S : Ensemble loc) :=
-    [ set l : loc | exists l' v, l' \in S /\ get l H = Some v /\ l' \in locs v].
 
+  (** The location that are pointed by location in S *)
+  Definition post (H : heap val) (S : Ensemble loc) :=
+    [ set l : loc | exists l' v, l' \in S /\ get l' H = Some v /\ l \in locs v].
+  
   (** TODO: move this to functions.v *)
-  Fixpoint app {A} (f : A -> A) n  : A ->  A :=
+
+  Fixpoint app {A} (f : A -> A) (n : nat) : A ->  A :=
     fun x =>
       match n with
-        | 0 => x
+        | 0%nat => x
         | S n' => f (app f n' x)
       end.
   
   Infix "^" := app (at level 30, right associativity) : fun_scope.
-
+  
+  Close Scope Z_scope.
+  
   Definition lfp {A} (f : Ensemble A -> Ensemble A) :=
     \bigcup_( n : nat ) ((f ^ n) (Empty_set A)).
   
   (** Least fixed point characterization of heap reachability. *)
   Definition reach (H : heap val) (Si : Ensemble loc) : Ensemble loc :=
     lfp (fun S => Union _ Si (post H S)).
+  
+  (** Alternative characterization of heap reachability. *)
+  Definition reach' (H : heap val) (Si : Ensemble loc) : Ensemble loc :=
+    \bigcup_( n : nat ) (((post H) ^ n) (Si)).
+  
+  (* The to definitions should be equivalent. TODO: Do the proof *)
+  Lemma reach_equiv H Si :
+    reach H Si <--> reach' H Si.
+  Proof.
+  Abort.
+  
+  (** A heap is well-formed if there are not dangling pointers in the stored values *)
+   Definition well_formed (S : Ensemble loc) (H : heap val) :=
+     forall l v, l \in S -> get l H = Some v -> locs v \subset dom H.
 
+   (** Well-formedness lifted to the environments. NOT USED *)
+   Definition well_formed_env S (H : heap val) (rho : env):=
+     forall x l, x \in S -> M.get x rho = Some l -> l \in dom H.
+   
+   (** A heap is closed in S if the locations of its image on S remain in S *)
+   Definition closed (S : Ensemble loc) (H : heap val) : Prop :=
+     forall l, l \in S -> exists v, get l H = Some v /\ locs v \subset S.
+
+   
+  (* The type of primitive operators *)
+  Definition prim : Type := list loc -> heap val -> option (loc * heap val).
+
+  Variable (pr : M.t prim).
   
   Fixpoint def_funs (B : fundefs) (l : loc) (rho : env) {struct B}
   : env :=
@@ -163,9 +358,7 @@ Module Sem (H : Heap).
         M.set f l (def_funs B' l rho)
       | Fnil => rho
     end.
-
-  Variable (pr : M.t (list loc -> heap val -> option (loc * heap val))).
-
+  
   Inductive big_step :
     heap val -> (* The heap. Maps locations to values *)
     env -> (* The environment. Maps variables to locations *)
@@ -173,14 +366,13 @@ Module Sem (H : Heap).
     res -> (* The location of the final result (?) *)
     nat -> (* The number of applications in the derivation *)
     nat -> (* The maximum space required for the evaluation *)
-    Prop :=
+    Type :=
   | Eval_constr :
       forall (H H' : heap val) (rho rho' : env) (x : var) (t : cTag) (ys :list var)
         (e : exp) (ls : list loc) (l : loc) (r : res) (c : nat) (m : nat),
         getlist ys rho = Some ls ->
         alloc (Vconstr t ls) H = (l, H') ->
-        M.set x l rho = rho' ->
-        big_step H' rho' e r c m ->
+        big_step H' (M.set x l rho) e r c m ->
         big_step H rho (Econstr x t ys e) r c m
   | Eval_proj :
       forall (H : heap val) (rho : env) (x : var) (t : cTag) (n : N)
@@ -217,14 +409,16 @@ Module Sem (H : Heap).
         setlist xs ls (def_funs B l rho') = Some rho'' ->
         big_step H rho'' e r c m ->
         big_step H rho (Eapp f t ys) r (c+1) m
-  | Eval_prim :
-      forall (H H' : heap val) (rho rho' : env) (x : var) (f : prim) f' (ys :list var)
-        (e : exp) (ls : list loc) (l : loc) (r : res) (c : nat) (m : nat),
-        getlist ys rho = Some ls ->
-        M.get f pr = Some f' ->
-        f' ls H = Some (l, H') -> 
-        big_step H' (M.set x l rho) e r c m ->
-        big_step H rho (Eprim x f ys e) r c m
+  (* Removing the primitive application rule. It requires adding axioms about
+     primitive operators. *)
+  (* | Eval_prim : *)
+  (*     forall (H H' : heap val) (rho : env) (x : var) f f' (ys :list var) *)
+  (*       (e : exp) (ls : list loc) (l : loc) (r : res) (c : nat) (m : nat), *)
+  (*       getlist ys rho = Some ls -> *)
+  (*       M.get f pr = Some f' -> *)
+  (*       f' ls H = Some (l, H') ->  *)
+  (*       big_step H' (M.set x l rho) e r c m -> *)
+  (*       big_step H rho (Eprim x f ys e) r c m *)
   | Eval_halt :
       forall H rho x l m,
         M.get x rho = Some l ->
@@ -236,10 +430,1781 @@ Module Sem (H : Heap).
         (* Whatever can be reached it can be reached from the H1 portion of the heap.
            Alternative (more direct?) characterization of garbage here
            might also be useful here *)
-        (reach H (image' (fun x => M.get x rho) (occurs_free e)) <-->
-         reach H1 (image' (fun x => M.get x rho) (occurs_free e))) ->
+        heap_eq (reach' H (env_locs rho (occurs_free e))) H H1 ->
         size H m' ->
         big_step H1 rho e r c m ->
         big_step H rho e r c (max m m').
+
+  (** * Lemmas about [post] and [reach'] *)
+  
+  Lemma post_heap_monotonic H1 H2 S :
+    H1 ⊑ H2 ->
+    post H1 S \subset post H2 S.
+  Proof.
+    unfold post. intros Hsub l [l' [v [Hin [Hget Hin']]]].
+    exists l', v. split; eauto.
+  Qed.
+  
+  Lemma post_set_monotonic S1 S2 H :
+    S1 \subset S2 ->
+    post H S1 \subset post H S2.
+  Proof.
+    unfold post. intros Hsub l [l' [v [Hin [Hget Hin']]]].
+    exists l', v. split; eauto.
+  Qed.
+
+  (* TODO move *) 
+  Lemma app_monotonic {A} (S1 S2 : Ensemble A) f n :
+    (forall S1 S2, S1 \subset S2 -> f S1 \subset f S2) ->
+    S1 \subset S2 ->
+    (f^n) S1 \subset (f^n) S2.
+  Proof.
+    induction n; intros H Hsub.
+    - eassumption.
+    - simpl. apply H. eapply IHn; eassumption.
+  Qed.
+
+  Open Scope program_scope.
+
+  Lemma compose_id_neut_l {A B} (f : A -> B) :
+    f_eq (id ∘ f) f.
+  Proof.
+    firstorder.
+  Qed.
+
+  Lemma compose_id_neut_r {A B} (f : A -> B) :
+    f_eq (f ∘ id) f.
+  Proof.
+    firstorder.
+  Qed.
+  
+  Lemma app_plus {A} (f : A -> A) m n :
+    f_eq (f ^ (m + n)) ((f ^ m) ∘ (f ^ n)).
+  Proof.
+    revert n; induction m; intros n; simpl.
+    - rewrite compose_id_neut_l. reflexivity.
+    - intros x. rewrite IHm. reflexivity.
+  Qed.
+
+  (* END *)
+
+  Lemma reach'_set_monotonic H S1 S2 :
+    S1 \subset S2 ->
+    reach' H S1 \subset reach' H S2.
+  Proof.
+    intros Hsub; intros x [i [_ Hin]]. 
+    exists i. split. constructor. eapply app_monotonic.
+    + intros. now eapply post_set_monotonic.
+    + eassumption.
+    + eassumption.
+  Qed.
+
+  Lemma reach'_extensive H S :
+    S \subset reach' H S.
+  Proof.
+    intros x Hin. exists 0; split; eauto.
+    now constructor.
+  Qed.
+  
+  Lemma Included_post_reach' H S :
+    (post H S) \subset reach' H S.
+  Proof.
+    intros x Hin. exists 1; split; eauto.
+    now constructor.
+  Qed.
+  
+  Lemma reach_unfold H S :
+    (reach' H S) <--> (Union _ S (reach' H (post H S))).
+  Proof.
+    split; intros x.
+    - intros [i [_ Hin]]. 
+      destruct i.
+      + eauto.
+      + right. exists i. split. now constructor.
+        replace ((post H ^ i) (post H S))
+        with (((post H ^ i) ∘ (post H ^ 1)) S) by eauto.
+        rewrite <- app_plus. rewrite plus_comm. eassumption.
+    - intros Hin. destruct Hin as [ x Hin | x [i [_ Hin]]].
+      + now eapply reach'_extensive.
+      + exists (i+1). split. now constructor.
+          rewrite app_plus. eassumption.
+  Qed.
+
+  (* TODO move *)
+  Lemma bigcup_merge {A} (F : nat -> Ensemble A) :
+    \bigcup_n (\bigcup_m (F (n + m))) <-->  \bigcup_n (F n).
+  Proof.
+    split; intros x [i [_ Hin]].
+    - destruct Hin as [j [_ Hin]].
+      exists (i + j). split; eauto. constructor.
+    - exists 0. split. now constructor. exists i.
+      split; eauto. constructor.
+  Qed.
+  (* END *)
+
+  (** reach is a post fixed point of post. Post is monotonic so
+      it is also a fixed point *)
+  Lemma reach'_post_fixed_point H S :
+    post H (reach' H S) \subset reach' H S.
+  Proof.
+    unfold post, reach'; simpl; intros x [l [v [[i [_ Hin]] Hin']]].
+    exists (i + 1). split. now constructor.
+    rewrite plus_comm, app_plus.
+    exists l, v. split; eauto.
+  Qed.
+  
+  Lemma reach'_post_fixed_point_n n H S :
+    (post H ^ n) (reach' H S) \subset reach' H S.
+  Proof.
+    induction n. 
+    - reflexivity.
+    - replace (Datatypes.S n) with (n + 1). rewrite app_plus.
+      eapply Included_trans.
+      eapply app_monotonic. now intros; eapply post_set_monotonic.
+      now apply reach'_post_fixed_point. eassumption.
+      omega.
+  Qed. 
+
+  (** [reach'] is idempotent *)
+  Lemma reach'_idempotent H S :
+    reach' H S <--> reach' H (reach' H S).
+  Proof.
+    unfold reach'. split; intros x Hin.
+    - exists 0. split. now constructor.
+      simpl. eassumption.
+    - rewrite <- bigcup_merge.
+      destruct Hin as [m [_ Hin]].
+      apply reach'_post_fixed_point_n in Hin.
+      exists 0. split; eauto. now constructor.
+  Qed.
+  
+  Lemma reach_spec H S S' :
+    S \subset S' -> S' \subset reach' H S ->
+    reach' H S <--> reach' H S'.
+  Proof.
+    intros Hsub1 Hsub2. split.
+    - eapply reach'_set_monotonic. eassumption.
+    - rewrite (reach'_idempotent H S).
+      apply reach'_set_monotonic. eassumption.
+  Qed.
+
+
+  (** Proper instances *)
+  Instance Proper_post : Proper (eq ==> Same_set loc ==> Same_set loc) post.
+  Proof.
+    intros x1 x2 Heq S1 S2 Heq'; subst; split; intros z [l [v [Hin [Hget Hin']]]].
+    repeat eexists; eauto; now rewrite <- Heq'; eauto.
+    repeat eexists; eauto; now rewrite Heq'; eauto.
+  Qed.
+
+  Lemma proper_post_n H n S1 S2 :
+    S1 <--> S2 ->
+    ((post H) ^ n) S1 <--> ((post H) ^ n) S2.
+  Proof.
+    induction n; eauto; intros Heq; simpl.
+    rewrite IHn; eauto. reflexivity.
+  Qed.
+
+  Instance Proper_reach' : Proper (eq ==> Same_set _ ==> Same_set _) reach'.
+  Proof.
+    intros H1 H2 heq S1 S2 Hseq; subst; split; intros x [n [Hn Hin]].
+    - eexists; split; eauto. eapply proper_post_n; eauto.
+      now symmetry.
+    - eexists; split; eauto. eapply proper_post_n; eauto.
+  Qed.
+  
+  Lemma post_heap_eq S H1 H2 :
+    S |- H1 ≡ H2 ->
+    post H1 S <--> post H2 S.
+  Proof.
+    intros Heq; split; intros x [l [v [Hin [Hget Hin']]]].
+    repeat eexists; eauto; now rewrite <- Heq; eauto.
+    repeat eexists; eauto; now rewrite Heq; eauto.
+  Qed.
+
+  
+  Lemma post_n_heap_eq n P H1 H2 :
+    reach' H1 P |- H1 ≡ H2 ->
+    (post H1 ^ n) P <--> (post H2 ^ n) P.
+  Proof.
+    induction n; intros Heq; try reflexivity.
+    simpl. rewrite IHn; eauto. apply post_heap_eq.
+    eapply heap_eq_antimon; eauto.
+    rewrite <- IHn; eauto. intros l Hin; eexists; split; eauto.
+    now constructor.
+  Qed.
+
+    Lemma post_n_heap_eq' n P H1 H2 :
+    reach' H2 P |- H1 ≡ H2 ->
+    (post H1 ^ n) P <--> (post H2 ^ n) P.
+  Proof.
+    induction n; intros Heq; try reflexivity.
+    simpl. rewrite IHn; eauto. apply post_heap_eq.
+    eapply heap_eq_antimon; eauto.
+    intros l Hin; eexists; split; eauto.
+    now constructor.
+  Qed.
+  
+  Lemma reach'_heap_eq P H1 H2 :
+    reach' H1 P |- H1 ≡ H2 ->
+    reach' H1 P <--> reach' H2 P.
+  Proof.
+    intros Heq; split; intros l [n [HT Hp]]; eexists; split; eauto;
+    try now eapply post_n_heap_eq; eauto.
+    eapply post_n_heap_eq'; eauto.
+    symmetry ; eauto.
+  Qed.  
+  
+  Lemma reach'_post S H : 
+    reach' H S <--> reach' H (Union loc S (post H S)).
+  Proof.
+    rewrite <- reach_spec with (S' := Union loc S (post H S)).
+    reflexivity.
+    now eauto with Ensembles_DB.
+    apply Union_Included. now apply reach'_extensive.
+    now apply Included_post_reach'.
+  Qed.
+
+  (** Reflexivity of [res_approx] *)
+  Lemma reach_res_approx H1 H2 S l n :
+    reach' H1 S <--> reach' H2 S ->
+    (reach' H1 S) |- H1 ≡ H2  ->
+    l \in S -> 
+    res_approx_fuel n (l, H1) (l, H2).
+  Proof.
+    intros Hr Hsub Hin. revert H1 H2 S l Hr Hsub Hin.
+    induction n using lt_wf_rec1; intros H1 H2 S l Hr Hsub Hin.
+    destruct n.
+    - simpl. intros. rewrite res_approx_fuel_eq; intros v Hget.
+      rewrite Hsub in Hget. eexists; split; eauto. destruct v.
+      split; eauto; intros. omega. split; eauto; intros; omega.
+      eapply reach'_extensive. eassumption.
+    - rewrite res_approx_fuel_eq; intros v Hget.
+      assert (Hget1 := Hget). rewrite Hsub in Hget. eexists; split; eauto. destruct v.
+      + split; eauto. intros i Hlt.
+        eapply Forall2_same.  intros l' Hin'.
+        eapply H with (S := Union _ S (post H1 S)); eauto.
+        rewrite <- reach_spec with (H := H1) (S := S).
+        rewrite <- reach_spec with (H := H2) (S := S).
+        eassumption. now eauto with Ensembles_DB.
+        apply Union_Included. now apply reach'_extensive.
+        eapply Included_trans with (s2 := post H2 S).
+        eapply (heap_eq_antimon) in Hsub; [| now apply reach'_extensive ].
+        rewrite post_heap_eq; eauto. reflexivity.
+        now apply Included_post_reach'.
+        now eauto with Ensembles_DB.
+        apply Union_Included. now apply reach'_extensive.
+        eapply Included_trans with (s2 := post H2 S).
+        eapply (heap_eq_antimon) in Hsub; [| now apply reach'_extensive ].
+        rewrite post_heap_eq; eauto. reflexivity.
+        rewrite Hr. now apply Included_post_reach'.
+        now rewrite <- reach'_post.
+        right. exists l. eexists. eauto.
+      + split; [ reflexivity |].
+        intros i x Hlt Hin'.
+        destruct (M.get x e) eqn:Heq.
+        * left; do 2 eexists. split; [| split ]; eauto.
+          eapply H with (S := Union _ S (post H1 S)); eauto.
+          rewrite <- reach_spec with (H := H1) (S := S).
+          rewrite <- reach_spec with (H := H2) (S := S).
+          eassumption. now eauto with Ensembles_DB.
+          apply Union_Included. now apply reach'_extensive.
+          eapply Included_trans with (s2 := post H2 S).
+          eapply (heap_eq_antimon) in Hsub; [| now apply reach'_extensive ].
+          rewrite post_heap_eq; eauto. reflexivity.
+          now apply Included_post_reach'.
+          now eauto with Ensembles_DB.
+          apply Union_Included. now apply reach'_extensive.
+          eapply Included_trans  with (s2 := post H2 S).
+          eapply (heap_eq_antimon) in Hsub; [| now apply reach'_extensive ].
+          rewrite post_heap_eq; eauto. reflexivity.
+          rewrite Hr. now apply Included_post_reach'.
+          now rewrite <- reach'_post.
+          right. exists l. eexists. repeat split; eauto.
+          exists x. split; eauto.
+        * right; eauto.
+      + eapply reach'_extensive. eassumption.
+  Qed.
+  
+  Corollary reach_res_equiv H1 H2 S l : 
+    reach' H1 S <--> reach' H2 S ->
+    (reach' H1 S) |- H1 ≡ H2 ->
+    l \in S -> 
+    (l, H1) ≈ (l, H2).
+  Proof.
+    intros Hr Hsub Hin n; split; rewrite <- res_approx_fuel_eq;
+    eapply reach_res_approx; eauto.
+    now symmetry. symmetry. rewrite <- Hr. eassumption.
+  Qed.
+
+  (* ΤODO move *)
+  Lemma Forall2_trans_strong (A : Type) (R1 R2 R3 : A -> A -> Prop) (l1 l2 l3 : list A) : 
+    (forall l1 l2 l3, R1 l1 l2 -> R2 l2 l3 -> R3 l1 l3) ->
+    Forall2 R1 l1 l2 -> Forall2 R2 l2 l3 -> Forall2 R3 l1 l3.
+  Proof.
+    intros H Hall1; revert l3; induction Hall1; intros l3 Hall2 ; eauto.
+    - inv Hall2. constructor.
+    - inv Hall2. constructor; eauto.
+  Qed.
+  
+  Lemma Preorder_res_equiv_fuel i : preorder res (res_approx_fuel i).
+  Proof.
+    constructor.
+    - induction i using lt_wf_rec1.
+      intros [l H1]. rewrite res_approx_fuel_eq. intros v Hget.
+      eexists; split; eauto. destruct v; split; eauto; intros.
+      + eapply Forall2_refl; intros l'. eapply H. eassumption.
+      + destruct (M.get x e) eqn:Hget'; eauto.
+        left; do 2 eexists; repeat split; eauto.
+        eapply H; eauto.
+    - induction i using lt_wf_rec1.
+      intros [l1 H1] [l2 H2] [l3 H3] Hap1 Hap2. rewrite res_approx_fuel_eq in *.
+      intros v1 Hget. edestruct Hap1 as [v2 [Hget2 Hval2]]. eassumption.
+      edestruct Hap2 as [v3 [Hget3 Hval3]]. eassumption.
+      eexists; split; eauto.
+      destruct v1; destruct v2; try contradiction; destruct v3; try contradiction.
+      + destruct Hval2 as [Heq2 Hlt2]. destruct Hval3 as [Heq3 Hlt3]. subst.
+        split; eauto; intros.
+        eapply Forall2_trans_strong; eauto. intros. eapply H. eassumption.
+        eapply H4. eapply H5.
+      + destruct Hval2 as [Heq2 Hlt2]. destruct Hval3 as [Heq3 Hlt3]. subst.
+        split; eauto; intros.
+        edestruct Hlt2 as [[l1' [l2' [Hgetl1 [Hgetl2 Hap1']]]] | [Hn1 Hn2]];
+          try eassumption;
+          edestruct Hlt3 as [[l3' [l4' [Hgetl3 [Hgetl4 Hap2']]]] | [Hn1' Hn2']];
+          try eassumption;
+          try congruence; try eassumption.
+        * left; repeat eexists; eauto.
+          rewrite Hgetl2 in Hgetl3; inv Hgetl3.
+          eapply H; eauto.
+        * right; eauto.
+  Qed.
+
+
+  Instance Reflexive_res_equiv_fuel i : Reflexive (res_approx_fuel i).
+  Proof.
+    eapply Preorder_res_equiv_fuel.
+  Qed.
+
+  Instance Transitive_res_equiv_fuel i : Transitive (res_approx_fuel i).
+  Proof.
+    eapply Preorder_res_equiv_fuel.
+  Qed.
+
+  Instance Equivalence_res_equiv : Equivalence res_equiv.
+  Proof.
+    constructor.
+    - intros res; split; rewrite <- res_approx_fuel_eq;
+      eapply Preorder_res_equiv_fuel.
+    - intros res res' H n. destruct (H n) as [H1 H2]. split; eauto.
+    - intros res1 res2 res3 H1 H2. intros n;
+      destruct (H1 n) as [Ht1 Ht2]; destruct (H2 n) as [Ht3 Ht4];
+      rewrite <- res_approx_fuel_eq in *. 
+      split. now eapply Preorder_res_equiv_fuel; eauto.
+      rewrite <- res_approx_fuel_eq. 
+      now eapply Preorder_res_equiv_fuel; eauto.
+  Qed.
+
+  Lemma reach_approx H1 H2 rho S : 
+    reach' H1 (image' (fun x => M.get x rho) S) <--> reach' H2 (image' (fun x => M.get x rho) S) ->
+    (reach' H1 (image' (fun x => M.get x rho) S)) |- H1 ≡ H2 -> 
+    heap_env_approx S (H2, rho) (H1, rho).
+  Proof.
+    intros Hreach Hsub x l Hin Hget. 
+    exists l. split. eassumption.
+    eapply reach_res_equiv. symmetry. eassumption.
+    symmetry. rewrite <- Hreach. eassumption.
+    eexists. split; eauto.
+  Qed.  
+
+ 
+  Corollary reach_heap_env_equiv H1 H2 rho S : 
+    reach' H1 (image' (fun x => M.get x rho) S) <--> reach' H2 (image' (fun x => M.get x rho) S) ->
+    (reach' H1 (image' (fun x => M.get x rho) S)) |- H1 ≡ H2 -> 
+    S |- (H1, rho) ⩪ (H2, rho).
+  Proof.
+    intros. split; eapply reach_approx; simpl; try eassumption.
+    symmetry. eassumption. rewrite <- H. now symmetry.
+  Qed.
+
+  Fixpoint noGC {Heap rho e v c m} (H : big_step Heap rho e v c m) : Prop :=
+    match H with
+      | Eval_constr Hp Hp' rho rho' x t ys e ls l r c m x0 x1 H' =>
+        noGC H'
+      | Eval_proj H rho x t n y e l l' ls r c m x0 x1 x2 H' =>
+        noGC H'
+      | Eval_case H rho y cl l t ls e r c m x x0 x1 H' =>
+        noGC H'
+      | Eval_fun Hp Hp' rho B l e r c m x H' =>
+        noGC H'
+      | Eval_app H rho rho' rho'' B f t xs e l ls ys r c m x x0 x1 x2 x3 H' =>
+        noGC H'
+      (* | Eval_prim H Hp' rho x f f' ys e ls l r c m x0 x1 x2 H' => *)
+      (*   noGC H' *)
+      | Eval_halt _ _ _ _ _ _ _ => True
+      | Eval_GC _ _ _ _ _ _ _ _ _ _ _ _ _ => False
+    end.
+
+   Fixpoint size_big_step {Heap rho e v c m} (H : big_step Heap rho e v c m) : nat :=
+    match H with
+      | Eval_constr Hp Hp' rho rho' x t ys e ls l r c m x0 x1 H' =>
+        S (size_big_step H')
+      | Eval_proj H rho x t n y e l l' ls r c m x0 x1 x2 H' =>
+        S (size_big_step H')
+      | Eval_case H rho y cl l t ls e r c m x x0 x1 H' =>
+        S (size_big_step H')
+      | Eval_fun Hp Hp' rho B l e r c m x H' =>
+        S (size_big_step H')
+      | Eval_app H rho rho' rho'' B f t xs e l ls ys r c m x x0 x1 x2 x3 H' =>
+        S (size_big_step H')
+      (* | Eval_prim H Hp' rho x f f' ys e ls l r c m x0 x1 x2 H' => *)
+      (*   S (size_big_step H')         *)
+      | Eval_halt _ _ _ _ _ _ _ => 0
+      | Eval_GC _ _ _ _ _ _ _ _ _ _ _ _ H' => S (size_big_step H')
+    end.
+   
+   
+   (** Well formedness preservation lemmas *)
+
+   Lemma alloc_dom_subset (H H' : heap val) (v : val) (l : loc) :
+     alloc v H = (l, H') ->
+     dom H \subset dom H'.
+   Proof.
+     intros Ha l' [y Hget].
+     destruct (loc_dec l l'); subst.
+     - eexists. erewrite gas; eauto.
+     - eexists. erewrite gao; eauto.
+   Qed.
+     
+   Definition well_formed_alloc S (H H' : heap val) (v : val) (l : loc) :
+     well_formed S H -> alloc v H = (l, H') ->
+     locs v \subset (dom H) ->
+     well_formed S H'.
+   Proof.
+     intros Hwf ha Hsub l' v' Sin Hget. destruct (loc_dec l l'); subst.
+     - erewrite gas in Hget; eauto. inv Hget.
+       eapply Included_trans. eassumption.
+       now eapply alloc_dom_subset; eauto.
+     - erewrite gao in Hget; eauto.
+       eapply Included_trans. now eauto.
+       now eapply alloc_dom_subset; eauto.
+   Qed.
+   
+   Definition well_formed_env_alloc_extend S (H H' : heap val) rho x (v : val) (l : loc) :
+     well_formed_env (Setminus _ S (Singleton _ x)) H rho -> alloc v H = (l, H') ->
+     locs v \subset (dom H) ->
+     well_formed_env S H' (M.set x l rho).
+   Proof.
+     intros Hwf ha Hsub x' l' Hin Hget. destruct (peq x x'); subst.
+     - rewrite M.gss in Hget. inv Hget.
+       eexists v. eapply gas. eauto.
+     - rewrite M.gso in Hget; eauto. 
+       eapply alloc_dom_subset; eauto. eapply Hwf; eauto.
+       constructor; eauto. intros Hc; inv Hc; congruence.
+   Qed.  
+
+   Lemma Forall2_monotonic_strong (A : Type) (R R' : A -> A -> Prop) (l1 l2 : list A) :
+     (forall x1 x2 : A, List.In x1 l1 -> List.In x2 l2 -> R x1 x2 -> R' x1 x2) ->
+     Forall2 R l1 l2 -> Forall2 R' l1 l2.
+   Proof.
+     revert l2.
+     induction l1 as [| x xs IHxs ]; intros l2 H Hall.
+     - inv Hall; eauto. 
+     - destruct l2; inv Hall. constructor; eauto.
+       eapply H; eauto. now constructor. now constructor.
+       eapply IHxs; eauto. intros. eapply H.
+       now constructor; eauto. now constructor; eauto.
+       eassumption.
+   Qed.
+
+   Lemma heap_env_approx_set S H1 H2 x l1 l2 rho1 rho2 :
+     heap_env_approx (Setminus _ S (Singleton _ x)) (H1, rho1) (H2, rho2) ->
+     (l1, H1) ≈ (l2, H2) ->
+     heap_env_approx S (H1, M.set x l1 rho1) (H2, M.set x l2 rho2).
+   Proof.
+     intros Heq Hreq. intros y l Hin Hget.
+     destruct (peq x y); subst; simpl in *. 
+     - exists l2. rewrite M.gss in *; inv Hget; eauto.
+     - rewrite M.gso in *; eauto. eapply Heq in Hget; eauto.
+       constructor; eauto. intros Hc; inv Hc; congruence.
+   Qed.
+
+
+
+   Lemma heap_env_equiv_set S H1 H2 x l1 l2 rho1 rho2 :
+     Setminus _ S (Singleton _ x) |- (H1, rho1) ⩪ (H2, rho2) ->
+     (l1, H1) ≈ (l2, H2) ->
+     S  |- (H1, M.set x l1 rho1) ⩪ (H2, M.set x l2 rho2).
+   Proof.
+     intros [Heq1 Heq2] Hreq. split.
+     now eapply heap_env_approx_set.
+     now eapply heap_env_approx_set; eauto; symmetry.
+   Qed.
+   
+   Instance Proper_heap_env_approx : Proper (Same_set _ ==> eq ==> eq ==> iff) heap_env_approx.
+   Proof.
+     intros s1 s2 hseq p1 p2 Heq p1' p2' Heq'; subst; split; intros H1;
+     destruct p2; destruct p2'; firstorder.
+   Qed.
+
+   Instance Proper_heap_env_equiv : Proper (Same_set _ ==> eq ==> eq ==> iff) heap_env_equiv.
+   Proof.
+     intros s1 s2 hseq p1 p2 Heq p1' p2' Heq'; subst.
+     split; intros [h1 h2]; split; (try now rewrite hseq; eauto);
+     rewrite <- hseq; eauto.
+   Qed.
+
+   Lemma heap_env_equiv_antimon S1 S2 H1 H2 rho1 rho2 :
+     S1 |- (H1, rho1) ⩪ (H2, rho2) ->
+     S2 \subset S1 ->
+     S2 |- (H1, rho1) ⩪ (H2, rho2).
+   Proof.
+     firstorder.
+   Qed.
+
+   Lemma heap_env_equiv_setlist S H1 H2 xs ls1 ls2 rho1 rho2 rho1' rho2' :
+     Setminus _ S (FromList xs) |- (H1, rho1) ⩪ (H2, rho2) ->
+     setlist xs ls1 rho1 = Some rho1' -> setlist xs ls2 rho2 = Some rho2' ->
+     Forall2 (fun l1 l2 => (l1, H1) ≈ (l2, H2)) ls1 ls2  ->
+     S  |- (H1, rho1') ⩪ (H2, rho2').
+   Proof with (now eauto with Ensembles_DB).
+     revert S rho1' rho2' ls1 ls2; induction xs;
+     intros S  rho1' rho2' ls1 ls2 Heq Hs1 Hs2 Hall.
+     - destruct ls1; destruct ls2; try discriminate. inv Hs1; inv Hs2; eauto.
+       rewrite FromList_nil, Setminus_Empty_set_neut_r in Heq. eassumption.
+     - destruct ls1; destruct ls2; try discriminate.
+       inv Hall. simpl in Hs1, Hs2.
+       destruct (setlist xs ls1 rho1) eqn:Hset1; try discriminate.
+       destruct (setlist xs ls2 rho2) eqn:Hset2; try discriminate.
+       inv Hs1; inv Hs2. eapply heap_env_equiv_set; eauto.
+       eapply IHxs; eauto. eapply heap_env_equiv_antimon; eauto.
+       rewrite FromList_cons...
+   Qed.
+
+   Lemma heap_env_equiv_def_funs S H1 H2 B l1 l2 rho1 rho2  :
+     Setminus _ S (name_in_fundefs B) |- (H1, rho1) ⩪ (H2, rho2) ->
+     (l1, H1) ≈ (l2, H2) ->
+     S  |- (H1, def_funs B l1 rho1) ⩪ (H2, def_funs B l2 rho2).
+   Proof with (now eauto with Ensembles_DB).
+     revert S; induction B;
+     intros S Heq Hreq.
+     - simpl. eapply heap_env_equiv_set; eauto.
+       eapply IHB; eauto. eapply heap_env_equiv_antimon; eauto.
+       simpl. rewrite Setminus_Union...
+     - simpl. rewrite Setminus_Empty_set_neut_r in Heq.
+       eassumption.
+   Qed.
+   
+   Lemma reachable_closed H S l v:
+     l \in reach' H S ->
+     get l H = Some v ->
+     locs v \subset reach' H S.
+   Proof.
+     intros Hin Hget.
+     eapply Included_trans;
+       [| now eapply reach'_post_fixed_point_n with (n := 1)]; simpl.
+     intros l' Hin'. do 2 eexists. split. eassumption. now split; eauto.
+   Qed.
+
+   Lemma reachable_in_dom H S :
+     well_formed (reach' H S) H ->
+     S \subset dom H ->
+     reach' H S \subset dom H.
+   Proof.
+     intros H1 Hs l [n [_ Hr]]. destruct n; eauto.
+     simpl in Hr. destruct Hr as [l' [v' [Hin [Hget Hin']]]].
+     eapply H1; eauto. eexists; split; eauto. now constructor; eauto.
+   Qed.
+
+   Lemma res_approx_weakening S1 S2 H1 H2 H1' H2' l1 l2 i :
+     closed S1 H1 -> closed S2 H2 ->
+     res_approx_fuel' i (l1, H1) (l2, H2) ->
+     H1 ⊑ H1' -> 
+     H2 ⊑ H2' ->
+     l1 \in S1 -> l2 \in S2 -> 
+     res_approx_fuel' i (l1, H1') (l2, H2').
+   Proof.
+     intros Hwf1 Hwf2 Heq Hsub1 Hsub2.
+     revert l1 l2 Heq; induction i using lt_wf_rec1; intros l1 l2 Heq Hdom1 Hdom2.
+     intros v1 Hget1. edestruct (Hwf1 _ Hdom1) as [v1' [Hget1' Hsub1']].
+     edestruct (Hwf2 _ Hdom2) as [v2' [Hget2' Hsub2']].
+     specialize (Hsub1 _ _ Hget1'). rewrite Hsub1 in Hget1; inv Hget1.
+     specialize (Hsub2 _ _ Hget2').
+     edestruct Heq as [v2 [Hget2 Hm]]; eauto. rewrite Hget2 in Hget2'; inv Hget2'.
+     eexists; split; [ now eauto |]. destruct v1; destruct v2'; try contradiction.
+     + inv Hm; split; eauto. intros i' Hlt.
+       eapply Forall2_monotonic_strong
+       with (R :=  fun l3 l4 => l3 \in S1 -> l4 \in S2 -> res_approx_fuel i' (l3, H1') (l4, H2')).
+       * intros l1' l2' Hin1 Hin2 Hyp. eapply Hyp; eauto.
+       * eapply Forall2_monotonic; [| eauto ].
+         intros. rewrite res_approx_fuel_eq. eapply H; eauto.
+         rewrite <- res_approx_fuel_eq. eassumption.
+     + inv Hm; split; eauto. intros i' x Hlt Hfv.
+       specialize (H3 i' x Hlt Hfv). inversion H3 as [[l3 [l4 [Hget3 [Hget4 Hres]]]] | H3']; eauto.
+       left. exists l3, l4. split; [| split ]; eauto.
+       rewrite res_approx_fuel_eq. eapply H; eauto.
+       rewrite <- res_approx_fuel_eq. eassumption.
+       eapply Hsub1'; eauto. eexists; split; eauto.
+       eapply Hsub2'; eauto. eexists; split; eauto.
+   Qed.
+
+   Lemma reach'_closed S H :
+     well_formed (reach' H S) H ->
+     S \subset dom H ->
+     closed (reach' H S) H.
+   Proof.
+     intros HHwf sub l Hreach.
+     edestruct reachable_in_dom as [v Hget]; eauto.
+     eexists; split; eauto.
+     eapply reachable_closed; eauto.
+   Qed.
+
+   Corollary res_equiv_weakening S1 S2 H1 H2 H1' H2' l1 l2 :
+     closed S1 H1 -> closed S2 H2 ->
+     (l1, H1) ≈ (l2, H2) ->
+     H1 ⊑ H1' ->
+     H2 ⊑ H2' ->
+     l1 \in S1 -> l2 \in S2 -> 
+     (l1, H1') ≈ (l2, H2').
+   Proof.
+     intros Hwf1 Hwf2 Heq Hsub1 Hsub2 Hin1 Hin2 i. destruct (Heq i) as [Heq1 He2].
+     split. now eapply (res_approx_weakening S1 S2 H1 H2 H1' H2'); eauto.
+     now eapply (res_approx_weakening S2 S1 H2 H1 H2' H1'); eauto.
+   Qed.
+
+   Lemma Forall2_symm (A : Type) (R : A -> A -> Prop) (l1 l2 : list A) : 
+     Symmetric R -> Forall2 R l1 l2 -> Forall2 R l2 l1.
+   Proof.
+     intros H Hall; induction Hall; eauto.
+   Qed.
+
+   Lemma Forall2_symm_strong (A : Type) (R1 R2 : A -> A -> Prop) (l1 l2 : list A) : 
+     (forall l1 l2, R1 l1 l2 -> R2 l2 l1) -> Forall2 R1 l1 l2 -> Forall2 R2 l2 l1.
+   Proof.
+     intros H Hall; induction Hall; eauto.
+  Qed.
+   
+   Lemma heap_env_approx_set_alloc_Vconstr S S1 S2 H1 H2 H1' H2' x t ls ls' l1 l2 rho1 rho2 :
+     closed S1 H1 -> closed S2 H2 ->
+     env_locs rho1 (Setminus _ S (Singleton _ x)) \subset S1 ->
+     env_locs rho2 (Setminus _ S (Singleton _ x)) \subset S2 ->
+     FromList ls \subset S1 ->
+     FromList ls' \subset S2 -> 
+     heap_env_approx (Setminus _ S (Singleton _ x)) (H1, rho1) (H2, rho2) ->
+     alloc (Vconstr t ls) H1 = (l1, H1') -> alloc (Vconstr t ls') H2 = (l2, H2') ->
+     Forall2 (fun l1 l2 => (l1, H1) ≈ (l2, H2)) ls ls' ->
+     heap_env_approx S (H1', (M.set x l1 rho1)) (H2', (M.set x l2 rho2)).
+   Proof.
+     intros Hwf1 Hwf2 He1 He2 Hl1 Hl2 Heq Hal1 Hal2 Hall; simpl; intros y l Hin Hget.
+     destruct (peq x y); subst.
+     + rewrite M.gss in *. inv Hget. eexists; split; eauto. split.
+       * intros v Hget. erewrite gas in *; eauto. inv Hget. eexists; split; eauto.
+         simpl. split; eauto. intros i Hlt.
+         eapply Forall2_monotonic_strong
+         with (R :=  fun l3 l4 => l3 \in S1 -> l4 \in S2 -> res_approx_fuel i (l3, H1') (l4, H2')).
+         intros l1' l2' Hin1 Hin2 Hyp. eapply Hyp; eauto.
+         eapply Forall2_monotonic; [| eauto ].
+         intros. rewrite res_approx_fuel_eq. eapply (res_approx_weakening _ _ H1 H2); eauto.
+         eapply H; eauto. now eapply alloc_subheap; eauto. now eapply alloc_subheap; eauto.
+       * intros v Hget. erewrite gas in *; eauto. inv Hget. eexists; split; eauto.
+         simpl. split; eauto. intros i Hlt.
+         eapply Forall2_monotonic_strong
+         with (R :=  fun l3 l4 => l3 \in S2 -> l4 \in S1 -> res_approx_fuel i (l3, H2') (l4, H1')).
+         intros l1' l2' Hin1 Hin2 Hyp. eapply Hyp; eauto.
+         eapply Forall2_symm_strong with (R2 := (fun l1 l2 : loc => (l1, H2) ≈ (l2, H1))) in Hall.
+         eapply Forall2_monotonic; [| eauto ].
+         intros. rewrite res_approx_fuel_eq. eapply (res_approx_weakening _ _ H2 H1); eauto.
+         eapply H; eauto. now eapply alloc_subheap; eauto. now eapply alloc_subheap; eauto.
+         intros; now symmetry.
+     + rewrite M.gso in *; eauto. assert (Hget1 := Hget). eapply Heq in Hget.
+       destruct Hget as [l' [Hget' Heq']]. eexists; split; eauto.
+       eapply (res_equiv_weakening _ _ H1 H2  H1' H2'); eauto; simpl in *.
+       now eapply alloc_subheap; eauto.
+       now eapply alloc_subheap; eauto.
+       eapply He1; eauto. repeat eexists; eauto.
+       intros Hc; inv Hc. congruence.
+       eapply He2; eauto. repeat eexists; eauto.
+       intros Hc; inv Hc. congruence.
+       econstructor; eauto. intros Hc; inv Hc; congruence.
+   Qed.
+
+   Corollary heap_env_equiv_set_alloc_Vconstr S S1 S2 H1 H2 H1' H2' x t ls ls' l1 l2 rho1 rho2 :
+     closed S1 H1 -> closed S2 H2 ->
+     env_locs rho1 (Setminus _ S (Singleton _ x)) \subset S1 ->
+     env_locs rho2 (Setminus _ S (Singleton _ x)) \subset S2 ->
+     FromList ls \subset S1 ->
+     FromList ls' \subset S2 ->
+     Setminus _ S (Singleton _ x) |- (H1, rho1) ⩪ (H2, rho2) ->
+     alloc (Vconstr t ls) H1 = (l1, H1') -> alloc (Vconstr t ls') H2 = (l2, H2') ->
+     Forall2 (fun l1 l2 => (l1, H1) ≈ (l2, H2)) ls ls' ->
+     S |- (H1', M.set x l1 rho1) ⩪ (H2', M.set x l2 rho2).
+   Proof.
+     intros Hwf1 Hwf2 Hwfe1 Hwfe2 Hl1 Hl2 [Heq1 Heq2] Hal1 Hal2 Hall; split.
+     now eapply (heap_env_approx_set_alloc_Vconstr _ _ _ H1 H2); eauto.
+     eapply (heap_env_approx_set_alloc_Vconstr _ _ _ H2 H1); eauto.
+     eapply Forall2_symm_strong; [| eassumption ]. intros; now symmetry; eauto.
+   Qed.
+   
+   Instance Equivalence_heap_env_equiv S : Equivalence (heap_env_equiv S).
+   Proof.
+     constructor.
+     - intros [H rho]; split; intros l Hget; eexists; split; eauto; reflexivity.
+     - intros [H rho] [H' rho'] H1; split; intros v l Hin Hget;
+       eapply H1; eauto.
+     - edestruct Equivalence_res_equiv; eauto.
+       intros [H rho] [H' rho'] [H'' rho''] H1 H2; split; intros v l Hin Hget.
+       edestruct H1 as [H1' _]; eauto. edestruct H1' as [v1 [Hget1 Hres1]]; eauto.
+       edestruct H2 as [H2' _]; eauto. edestruct H2' as [v2 [Hget2 Hres2]]; eauto.
+       edestruct H2 as [_ H2']; eauto. edestruct H2' as [v2 [Hget2 Hres2]]; eauto.
+       edestruct H1 as [_ H1']; eauto. edestruct H1' as [v1 [Hget1 Hres1]]; eauto.
+   Qed.
+   
+   Lemma heap_env_approx_set_alloc_Vfun S S1 S2 H1 H2 H1' H2' x B l1 l2 rho1 rho2 :
+     closed S1 H1 -> closed S2 H2 ->
+     env_locs rho1 (Setminus _ S [set x]) \subset S1 ->
+     env_locs rho2 (Setminus _ S [set x]) \subset S2 ->
+     (occurs_free_fundefs B) \subset (Setminus _ S [set x]) ->
+     Setminus _ S [set x] |- (H1, rho1) ⩪ (H2, rho2) ->
+     alloc (Vfun rho1 B) H1 = (l1, H1') -> alloc (Vfun rho2 B) H2 = (l2, H2') ->
+     heap_env_approx S (H1', (M.set x l1 rho1)) (H2', (M.set x l2 rho2)).
+   Proof.
+     intros Hwf1 Hwf2 He1 He2 Hsub [Heq1 Heq2] Hal1 Hal2 y l Hin Hget; simpl.
+     destruct (peq x y); subst.
+     - rewrite M.gss in *. inv Hget. eexists; split; eauto. split.
+       + intros v Hget. erewrite gas in *; eauto. inv Hget. eexists; split; eauto.
+         simpl. split; eauto. intros i x Hlt Hin'.
+         destruct (M.get x rho1) eqn:Hget.
+         * edestruct Heq1 as [x' [Hget' Heq']]; eauto.
+           left. repeat eexists; eauto. rewrite res_approx_fuel_eq.
+           eapply (res_approx_weakening _ _ H1 H2); eauto.
+           now destruct (Heq' i); eauto. 
+           now eapply alloc_subheap; eauto.
+           now eapply alloc_subheap; eauto. 
+           eapply He1. now eexists; split; eauto.
+           eapply He2. now eexists; split; eauto.
+         * right; split; eauto.
+           destruct (M.get x rho2) eqn:Hget'; eauto.
+           edestruct Heq2 as [x' [Hget'' Heq']]; eauto; congruence.
+       + intros v Hget. erewrite gas in *; eauto. inv Hget. eexists; split; eauto.
+         simpl. split; eauto. intros i x Hlt Hin'.
+         destruct (M.get x rho1) eqn:Hget.
+         * edestruct Heq1 as [x' [Hget' Heq']]; eauto.
+           left. repeat eexists; eauto. rewrite res_approx_fuel_eq.
+           symmetry in Heq'. eapply (res_approx_weakening _ _ H2 H1); eauto.
+           now destruct (Heq' i); eauto. 
+           now eapply alloc_subheap; eauto.
+           now eapply alloc_subheap; eauto. 
+           eapply He2. now eexists; split; eauto.
+           eapply He1. now eexists; split; eauto.
+         * right; split; eauto.
+           destruct (M.get x rho2) eqn:Hget'; eauto.
+           edestruct Heq2 as [x' [Hget'' Heq']]; eauto; congruence.
+     - rewrite M.gso in *; eauto. assert (Hget1 := Hget). eapply Heq1 in Hget.
+       destruct Hget as [l' [Hget' Heq']]. eexists; split; eauto.
+       eapply (res_equiv_weakening _ _ H1 H2  H1' H2'); eauto; simpl in *.
+       now eapply alloc_subheap; eauto.
+       now eapply alloc_subheap; eauto.
+       eapply He1; eauto. repeat eexists; eauto.
+       intros Hc; inv Hc. congruence.
+       eapply He2; eauto. repeat eexists; eauto.
+       intros Hc; inv Hc. congruence.
+       econstructor; eauto. intros Hc; inv Hc; congruence.
+   Qed.
+
+   Corollary heap_env_equic_set_alloc_Vfun S S1 S2 H1 H2 H1' H2' x B l1 l2 rho1 rho2 :
+     closed S1 H1 -> closed S2 H2 ->
+     env_locs rho1 (Setminus _ S [set x]) \subset S1 ->
+     env_locs rho2 (Setminus _ S [set x]) \subset S2 ->
+     (occurs_free_fundefs B) \subset (Setminus _ S [set x]) ->
+     Setminus _ S [set x] |- (H1, rho1) ⩪ (H2, rho2) ->
+     alloc (Vfun rho1 B) H1 = (l1, H1') -> alloc (Vfun rho2 B) H2 = (l2, H2') ->
+     S |- (H1', (M.set x l1 rho1)) ⩪ (H2', (M.set x l2 rho2)).
+   Proof.
+     intros Hwf1 Hwf2 Hwfe1 Hwfe2 Hsub Heq Hal1 Hal2; split.
+     now eapply (heap_env_approx_set_alloc_Vfun _ _ _ H1 H2); eauto.
+     eapply (heap_env_approx_set_alloc_Vfun _ _ _ H2 H1); eauto.
+     symmetry; eauto.
+   Qed.
+
+   Lemma heap_env_approx_alloc_Vfun S S1 S2 H1 H2 H1' H2' B l1 l2 rho1 rho2 :
+     closed S1 H1 -> closed S2 H2 ->
+     env_locs rho1 S \subset S1 ->
+     env_locs rho2 S \subset S2 ->
+     S |- (H1, rho1) ⩪ (H2, rho2) ->
+     alloc (Vfun rho1 B) H1 = (l1, H1') -> alloc (Vfun rho2 B) H2 = (l2, H2') ->
+     heap_env_approx S (H1', rho1) (H2', rho2).
+   Proof.
+     intros Hwf1 Hwf2 He1 He2  [Heq1 Heq2] Hal1 Hal2 y l Hin Hget; simpl.
+     edestruct Heq1 as [x' [Hget' Heq']]; eauto.
+     eexists; split; eauto.
+     eapply (res_equiv_weakening _ _ H1 H2); eauto.
+     now eapply alloc_subheap; eauto.
+     now eapply alloc_subheap; eauto. 
+     eapply He1. now eexists; split; eauto.
+     eapply He2. now eexists; split; eauto.
+   Qed.
+
+   Corollary heap_env_equiv_alloc_Vfun S S1 S2 H1 H2 H1' H2' B l1 l2 rho1 rho2 :
+     closed S1 H1 -> closed S2 H2 ->
+     env_locs rho1 S \subset S1 ->
+     env_locs rho2 S \subset S2 ->
+     S |- (H1, rho1) ⩪ (H2, rho2) ->
+     alloc (Vfun rho1 B) H1 = (l1, H1') -> alloc (Vfun rho2 B) H2 = (l2, H2') ->
+     S |- (H1', rho1) ⩪ (H2', rho2).
+   Proof.
+     intros. split.
+     now eapply (heap_env_approx_alloc_Vfun _ _ _ H1 H2); eauto.
+     now eapply (heap_env_approx_alloc_Vfun _ _ _ H2 H1); eauto; symmetry.
+   Qed.
+   
+   Lemma env_locs_monotonic S1 S2 rho :
+     S1 \subset S2 ->
+     env_locs rho S1 \subset env_locs rho S2.
+   Proof.
+     firstorder.
+   Qed.
+
+   Instance Proper_env_locs : Proper (eq ==> Same_set _ ==> Same_set _) env_locs.
+   Proof.
+     intros rho1 rho2 heq s1 s2 Hseq; subst.
+     firstorder.
+   Qed.
+  
+
+   
+   Lemma heap_env_equiv_def_funs_alloc S S1 S2 H1 H2 H1' H2' B B' l1 l2 rho1 rho2 :
+     closed S1 H1 -> closed S2 H2 ->
+     env_locs rho1 (Setminus _ S (name_in_fundefs B)) \subset S1 ->
+     env_locs rho2 (Setminus _ S (name_in_fundefs B)) \subset S2 ->
+     (occurs_free_fundefs B') \subset (Setminus _ S (name_in_fundefs B)) -> 
+     (Setminus _ S (name_in_fundefs B)) |- (H1, rho1) ⩪ (H2, rho2) ->
+     alloc (Vfun rho1 B') H1 = (l1, H1') -> alloc (Vfun rho2 B') H2 = (l2, H2') ->
+     S |- (H1', def_funs B l1 rho1) ⩪ (H2', def_funs B l2 rho2).
+   Proof with now eauto with Ensembles_DB.
+     intros Hwf1 Hwf2 He1 He2 Hsub Heq Hal1 Hal2.
+     revert S He1 He2 Hsub Heq; induction B; intros S He1 He2 Hsub Heq.
+     - eapply heap_env_equiv_set; eauto.
+       + simpl in *. eapply IHB; eauto.
+         eapply Included_trans; eauto.
+         eapply env_locs_monotonic...
+         eapply Included_trans; eauto.
+         eapply env_locs_monotonic...
+         eapply Included_trans; eauto...
+         eapply heap_env_equiv_antimon; eauto...
+       + destruct Heq as [Heq1 Heq2]. split.
+         { intros v1. erewrite !gas; eauto.
+           intros Hget; eexists; split; eauto.
+           inv Hget. split; eauto.
+           intros i x Hlt Hin.
+           destruct (M.get x rho1) eqn:Hget.
+           - edestruct Heq1 as [x' [Hget' Heq']]; eauto.
+             left. repeat eexists; eauto. rewrite res_approx_fuel_eq.
+             symmetry in Heq'. eapply (res_approx_weakening _ _ H1 H2); eauto.
+             now destruct (Heq' i); eauto. 
+             now eapply alloc_subheap; eauto.
+             now eapply alloc_subheap; eauto. 
+             eapply He1. now eexists; split; eauto.
+             eapply He2. now eexists; split; eauto.
+           - right; split; eauto.
+             destruct (M.get x rho2) eqn:Hget'; eauto.
+             edestruct Heq2 as [x' [Hget'' Heq']]; eauto; congruence. }
+         { intros v1. erewrite !gas; eauto.
+           intros Hget; eexists; split; eauto.
+           inv Hget. split; eauto.
+           intros i x Hlt Hin.
+           destruct (M.get x rho1) eqn:Hget.
+           - edestruct Heq1 as [x' [Hget' Heq']]; eauto.
+             left. repeat eexists; eauto. rewrite res_approx_fuel_eq.
+             symmetry in Heq'. eapply (res_approx_weakening _ _ H2 H1); eauto.
+             now destruct (Heq' i); eauto. 
+             now eapply alloc_subheap; eauto.
+             now eapply alloc_subheap; eauto. 
+             eapply He2. now eexists; split; eauto.
+             eapply He1. now eexists; split; eauto.
+           - right; split; eauto.
+             destruct (M.get x rho2) eqn:Hget'; eauto.
+             edestruct Heq2 as [x' [Hget'' Heq']]; eauto; congruence. }
+     - simpl in *. rewrite !Setminus_Empty_set_neut_r in He1, He2, Heq.
+       eapply (heap_env_equiv_alloc_Vfun _ _ _ H1 H2); eauto.
+   Qed.
+   
+   Lemma well_formed_env_antimon S1 S2 H rho :
+     well_formed_env S1 H rho ->
+     S2 \subset S1 ->
+     well_formed_env S2 H rho.
+   Proof.
+     firstorder.
+   Qed.
+
+   Lemma getlist_in_dom S H rho ys ls :
+     well_formed_env S H rho ->
+     getlist ys rho = Some ls ->
+     FromList ys \subset S ->
+     FromList ls \subset dom H. 
+   Proof.
+     revert ls; induction ys; intros ls Hwf Hget Hin; destruct ls; simpl in *; try discriminate.
+     - now eauto with Ensembles_DB.
+     - now eauto with Ensembles_DB.
+     - rewrite !FromList_cons in Hin. rewrite FromList_cons.
+       destruct (M.get a rho) eqn:Hgeta; try discriminate.
+       destruct (getlist ys rho) eqn:Hgetys; try discriminate.
+       inv Hget. eapply Union_Included.
+       eapply Singleton_Included. eapply Hwf; eauto. 
+       eapply IHys; eauto. eapply Included_trans; now eauto with Ensembles_DB.
+   Qed.
+
+   Lemma heap_env_equiv_getlist_Forall2 S H1 H2 ys ls1 ls2 rho1 rho2 :
+     S |- (H1, rho1) ⩪ (H2, rho2) ->
+     FromList ys \subset S ->
+     getlist ys rho1 = Some ls1 ->
+     getlist ys rho2 = Some ls2 ->
+     Forall2 (fun l1 l2 : loc => (l1, H1) ≈ (l2, H2)) ls1 ls2.
+   Proof.
+     revert ls1 ls2; induction ys; intros ls1 ls2 Heq Hin Hg1 Hg2;
+     destruct ls1; destruct ls2; simpl in *; try discriminate; try now constructor.
+     - destruct (M.get a rho1) eqn:Heqa;
+       destruct (getlist ys rho1) eqn:Heqys; try discriminate.
+     - destruct (M.get a rho2) eqn:Heqa;
+       destruct (getlist ys rho2) eqn:Heqys; try discriminate.
+     - rewrite FromList_cons in Hin.
+       destruct (M.get a rho1) eqn:Heqa;
+         destruct (getlist ys rho1) eqn:Heqys; try discriminate. inv Hg1.
+       eapply Heq in Heqa. destruct Heqa as [l' [Hget Heq']]. rewrite Hget in Hg2.
+       destruct (getlist ys rho2) eqn:Heqys'; try discriminate. inv Hg2.
+       constructor; eauto. eapply IHys; eauto.
+       eapply Included_trans; now eauto with Ensembles_DB.
+       eapply Included_trans; now eauto with Ensembles_DB.
+   Qed.
+   
+   Lemma env_locs_set_not_In S rho x l :
+     ~ x \in S ->
+     env_locs (M.set x l rho) S <--> env_locs rho S.
+   Proof.
+     intros Hin; split; intros l' H1.
+     - destruct H1 as [z [H1 H2]].
+       destruct (peq z x); subst.
+       + contradiction.
+       + rewrite M.gso in *; eauto. eexists; eauto.
+     - destruct H1 as [z [H1 H2]].
+       destruct (peq z x); subst.
+       + contradiction.
+       + eexists. rewrite M.gso; eauto.
+   Qed.
+
+   Lemma env_locs_set S rho x l :
+     x \in S ->
+     env_locs (M.set x l rho) S <--> Union _ [set l] (env_locs rho (Setminus _ S [set x])).
+   Proof.
+     intros Hin; split; intros l' H1.
+     - destruct H1 as [z [H1 H2]].
+       destruct (peq z x); subst.
+       + rewrite M.gss in *. inv H2; eauto.
+       + rewrite M.gso in *; eauto. right. eexists; split; eauto.
+         constructor; eauto. intros Hc; inv Hc; eauto.
+     - inv H1. eexists; split; eauto. inv H; now rewrite M.gss; eauto.
+       destruct H as [z [H1 H2]]. inv H1.
+       destruct (peq z x); subst.
+       + exfalso; eauto.
+       + eexists. rewrite M.gso; eauto.
+   Qed.
+
+   Lemma env_locs_set_Inlcuded S rho x l :
+     env_locs (M.set x l rho) (Union _ S [set x]) \subset
+     Union _ [set l] (env_locs rho S).
+   Proof.
+     intros l' H1.
+     - destruct H1 as [z [H1 H2]].
+       destruct (peq z x); subst.
+       + rewrite M.gss in *. inv H2; eauto.
+       + rewrite M.gso in *; eauto. right. eexists; split; eauto.
+         inv H1; eauto. inv H. congruence.
+   Qed.
+
+   Lemma env_locs_def_funs_Included B l rho S :
+     env_locs (def_funs B l rho)
+              (Union M.elt S (name_in_fundefs B)) \subset
+     Union _ (env_locs rho S) [set l].
+   Proof.
+     induction B; simpl.
+     - eapply Included_trans.
+       rewrite (Union_commut [set v]), Union_assoc.
+       eapply env_locs_set_Inlcuded. rewrite Union_commut.
+       eapply Union_Included; eauto with Ensembles_DB.
+     - rewrite Union_Empty_set_neut_r; eauto with Ensembles_DB.
+   Qed.
+
+   Lemma env_locs_set_list_Included ys ls rho rho' S :
+     setlist ys ls rho = Some rho'  ->
+     env_locs rho'
+              (Union M.elt S (FromList ys)) \subset
+     Union _ (env_locs rho S) (FromList ls).
+   Proof with now eauto with Ensembles_DB.
+     revert rho' S ls; induction ys; intros rho' S ls Hset.
+     - rewrite FromList_nil, Union_Empty_set_neut_r. inv Hset.
+       destruct ls; try discriminate. inv H0...
+     - destruct ls; try discriminate. simpl in *.
+       destruct (setlist ys ls rho) eqn:Hset'; try discriminate.
+       inv Hset. rewrite !FromList_cons.
+       rewrite (Union_commut [set a]), !Union_assoc. 
+       eapply Included_trans. eapply env_locs_set_Inlcuded.
+       eapply Union_Included; eauto with Ensembles_DB. 
+       eapply Included_trans. eapply IHys; eauto.
+       now eauto with Ensembles_DB. 
+   Qed.
+
+   Lemma alloc_Same_set {A} H (v : A) l H' :
+     alloc v H = (l, H') ->
+     dom H' <--> Union _ [set l] (dom H).
+   Proof. 
+     intros Ha; split; intros l' Hl'. 
+     - destruct Hl' as [v' Hget].
+       destruct (loc_dec l l'); subst; eauto.
+       right. eexists. erewrite <- gao; eauto.
+     - inv Hl'.
+       + inv H0. eexists; erewrite gas; eauto.
+       + destruct H0 as [v' Hget].
+         eexists v'. erewrite gao; eauto.
+         intros Hc; subst. erewrite alloc_fresh in Hget; eauto.
+         discriminate.
+   Qed.
+
+
+
+
+   Lemma post_Union H S1 S2 :
+     post H (Union _ S1 S2) <--> Union _ (post H S1) (post H S2).
+   Proof with now eauto with Ensembles_DB.
+     split; intros l Hp.
+     - destruct Hp as [l' [v [Hin [Hget Hin']]]].
+       inv Hin; [left | right ]; repeat eexists; eauto.
+     - destruct Hp as [ Hp | Hp ];
+       eapply post_set_monotonic; eauto...
+   Qed.
+
+   Lemma post_n_Union n H S1 S2 :
+     (post H ^ n) (Union _ S1 S2) <--> Union _ ((post H ^ n) S1) ((post H ^ n) S2).
+   Proof with now eauto with Ensembles_DB.
+     induction n;  try now firstorder.
+     simpl. rewrite IHn, post_Union. reflexivity.
+   Qed.
+
+   Lemma reach'_Union H S1 S2 :
+     reach' H (Union _ S1 S2) <--> Union _ (reach' H S1) (reach' H S2).
+   Proof.
+     split; intros l Hp.
+     - destruct Hp as [n [HT Hp]].
+       eapply post_n_Union in Hp. destruct Hp as [Hp | Hp ].
+       now left; firstorder. now right; firstorder.
+     - destruct Hp as [ l [n [HT Hp]] | l [n [HT Hp]] ];
+       repeat eexists; eauto; eapply post_n_Union; eauto.
+   Qed.
+
+   Lemma post_n_heap_monotonic n (H1 H2 : heap val) (S : Ensemble loc) :
+     H1 ⊑ H2 -> (post H1 ^ n) S \subset (post H2 ^ n) S.
+   Proof.
+     induction n; simpl; eauto with Ensembles_DB.
+     intros Hsub. eapply Included_trans.
+     eapply post_set_monotonic. now eauto.
+     now eapply post_heap_monotonic.
+   Qed.
+
+   Lemma reach'_heap_monotonic (H1 H2 : heap val) (S : Ensemble loc) :
+     H1 ⊑ H2 -> reach' H1 S \subset reach' H2 S.
+   Proof.
+     intros Hsub l [n [HT Hp]]. exists n; split; eauto.
+     eapply post_n_heap_monotonic; eauto.
+   Qed.
+
+    Lemma post_alloc S H v l H'  :
+     alloc v H = (l, H') ->
+     post H' S \subset (Union _ (post H S) (locs v)).
+    Proof.
+     intros Ha l' Hp.
+     destruct Hp as [l2 [v' [Hin2 [Hget Hin1]]]].
+     destruct (loc_dec l l2); subst; eauto.
+     + repeat eexists; eauto. erewrite gas in Hget; eauto.
+       inv Hget. eauto.
+     + left; repeat eexists; eauto. erewrite <-gao; eauto.
+    Qed.
+
+    Lemma post_n_alloc n S H v l H'  :
+      alloc v H = (l, H') ->
+      locs v \subset reach' H S ->
+      (post H' ^ n) S \subset reach' H S.
+    Proof.
+      revert S.
+      induction n; intros S Ha Hin; simpl; eauto with Ensembles_DB.
+      - now apply reach'_extensive.
+      - eapply Included_trans. eapply post_set_monotonic.
+        now eauto. eapply Included_trans. now eapply post_alloc; eauto.
+        eapply Union_Included. now eapply reach'_post_fixed_point_n with (n := 1).
+        eapply Included_trans; eauto. reflexivity.
+    Qed.
+
+   Lemma reach'_alloc S H v l H'  :
+     alloc v H = (l, H') ->
+     locs v \subset reach' H S ->
+     reach' H' S <--> reach' H S.
+   Proof.
+     intros Ha Hin.
+     split.
+     - intros l' [n [_ Hp]]. eapply post_n_alloc; eauto.
+     - eapply reach'_heap_monotonic. now eapply alloc_subheap; eauto.
+   Qed.
+
+   Instance Proper_well_formed : Proper (Same_set _ ==> eq ==> iff) well_formed.
+   Proof.
+     intros s1 s2 hseq H1 h2 Heq; subst. firstorder.
+   Qed.
+
+   Lemma well_formed_antimon S1 S2 H :
+     S1 \subset S2 ->
+     well_formed S2 H ->
+     well_formed S1 H.
+   Proof.
+     firstorder.
+   Qed.
+
+   Lemma post_Empty S H :
+     Disjoint _ S (dom H) ->
+     post H S <--> Empty_set _.
+   Proof.
+     intros Hd; split; eauto with Ensembles_DB.
+     intros l [l' [v [Hin [Hget _]]]].
+     exfalso. eapply Hd. constructor; eauto.
+     eexists; eauto.
+   Qed.
+
+   Lemma post_n_Disjoint n S H :
+     Disjoint _ S (dom H) ->
+     (post H ^ n) S \subset S.
+   Proof with now eauto with Ensembles_DB.
+     revert S; induction n; intros S Hd; eauto with Ensembles_DB.
+     replace (Datatypes.S n) with (n + 1) by omega.
+     rewrite app_plus. simpl. unfold compose.
+     eapply Included_trans. eapply proper_post_n.
+     rewrite post_Empty; eauto. reflexivity.
+     eapply Included_trans; [ eapply IHn | ]...
+   Qed.
+
+   Lemma reach'_Disjoint S H :
+     Disjoint _ S (dom H) ->
+     reach' H S <--> S.
+   Proof.
+     split.
+     - intros l [n [_ Hp]]. eapply post_n_Disjoint; eauto.
+     - apply reach'_extensive.
+   Qed.
+
+   Lemma well_formed_Union S1 S2 H :
+     well_formed S1 H ->
+     well_formed S2 H ->
+     well_formed (Union _ S1 S2) H.
+   Proof.
+     intros Hwf1 Hwf2 l v Hin Hget; inv Hin; eauto.
+   Qed.
+
+   Lemma env_locs_Union rho S1 S2 :
+     env_locs rho (Union _ S1 S2) <-->
+     Union _ (env_locs rho S1) (env_locs rho S2).
+   Proof.
+     split; intros l.
+     - intros [v [Hin Hget]]. inv Hin; firstorder.
+       now left; repeat eexists; eauto.
+       now right; repeat eexists; eauto.
+     - intros [ l' [v [Hin Hget]] | l' [v [Hin Hget]] ];
+       repeat eexists; eauto.
+   Qed.
+
+   Lemma well_formed_reach_alloc S H x l v H' rho :
+     well_formed (reach' H (env_locs rho S)) H ->
+     env_locs rho S \subset dom H ->
+     alloc v H = (l, H') ->
+     locs v \subset (reach' H (env_locs rho S)) ->
+     well_formed (reach' H' (env_locs (M.set x l rho) (Union _ S [set x]))) H'.
+   Proof with now eauto with Ensembles_DB.
+     intros Hwf Hsub Ha Hin.
+     eapply well_formed_antimon.
+     eapply reach'_set_monotonic. now eapply env_locs_set_Inlcuded.
+     rewrite reach'_alloc; eauto.
+     - rewrite reach'_Union. eapply well_formed_Union.
+       + rewrite reach'_Disjoint.
+         * intros l' v' Hin' Hget. inv Hin'.
+           erewrite gas in Hget; eauto. inv Hget.
+           eapply Included_trans; eauto.
+           eapply Included_trans;
+             [| now eapply dom_subheap; eapply alloc_subheap; eauto ].
+           eapply reachable_in_dom; eauto.
+         * constructor. intros l' Hc. inv Hc. inv H0.
+           destruct H1 as [v' Hget]. erewrite alloc_fresh in Hget; eauto.
+           discriminate.
+       + eapply well_formed_alloc; eauto.
+         eapply Included_trans; eauto. eapply reachable_in_dom; eauto.
+     - rewrite reach'_Union. eapply Included_Union_preserv_r.
+       eassumption.
+   Qed.
+
+   Lemma well_formed_reach_set S H x l rho :
+     well_formed (reach' H (env_locs rho S)) H ->
+     well_formed (reach' H [set l]) H ->
+     well_formed (reach' H (env_locs (M.set x l rho) (Union _ S [set x]))) H.
+   Proof with now eauto with Ensembles_DB.
+     intros Hwf  Hin.
+     eapply well_formed_antimon.
+     eapply reach'_set_monotonic. now eapply env_locs_set_Inlcuded.
+     rewrite reach'_Union. eapply well_formed_Union; eauto.
+   Qed.
+
+   Lemma env_locs_Empty S :
+     Empty_set _ <--> env_locs (M.empty _) S.
+   Proof.
+     split; eauto with Ensembles_DB.
+     intros l [v [Hs Hp]]. rewrite M.gempty in Hp.
+     discriminate.
+   Qed.
+
+   Lemma env_locs_singleton x l :
+     [set l] <--> env_locs (M.set x l (M.empty _)) (Union _ (Empty_set _) [set x]).
+   Proof.
+     rewrite env_locs_set; eauto with Ensembles_DB.
+     rewrite <- env_locs_Empty; eauto with Ensembles_DB.
+   Qed.
+
+    Lemma env_locs_singleton_Included x l rho S:
+     [set l] \subset env_locs (M.set x l rho) (Union _ S [set x]).
+   Proof.
+     rewrite env_locs_set; eauto with Ensembles_DB.
+   Qed.
+     
+   Lemma well_formed_reach_alloc_def_funs S H B l v H' rho :
+     well_formed (reach' H (env_locs rho S)) H ->
+     env_locs rho S \subset dom H ->
+     alloc v H = (l, H') ->
+     locs v \subset (reach' H (env_locs rho S)) ->
+     well_formed (reach' H' (env_locs (def_funs B l rho) (Union _ S (name_in_fundefs B)))) H'.
+   Proof with now eauto with Ensembles_DB.
+     induction B; intros Hwf Hsub Ha Hin; simpl.
+     - rewrite (Union_commut [set v0]), Union_assoc.
+       eapply well_formed_reach_set.
+       + eapply IHB; eauto.
+       + eapply well_formed_antimon.
+         eapply reach'_set_monotonic.
+         now apply env_locs_singleton_Included with (x := v0).
+         eapply well_formed_reach_alloc; eauto.
+     - rewrite Union_Empty_set_neut_r.
+       rewrite reach'_alloc; eauto.
+       eapply well_formed_alloc; eauto.
+       eapply Included_trans. eassumption.
+       eapply reachable_in_dom; eauto.
+   Qed.
+
+  Lemma occurs_free_Econstr_Included' (x : var) (t : cTag) (ys : list var) (e : exp) :
+    Setminus _ (occurs_free e) [set x] \subset
+    occurs_free (Econstr x t ys e).
+  Proof.
+    eapply Setminus_Included_Included_Union.
+    now apply occurs_free_Econstr_Included.
+  Qed.
+
+  Lemma FromList_env_locs xs ls rho S :
+    getlist xs rho = Some ls ->
+    FromList xs \subset S ->
+    FromList ls \subset env_locs rho S.
+  Proof with now eauto with Ensembles_DB.
+    revert ls; induction xs; intros ls Hget Hs; simpl in *.
+    - inv Hget. rewrite FromList_nil...
+    - destruct (M.get a rho) eqn:Hgeta; try discriminate.
+      destruct (getlist xs rho) eqn:Hgetl; try discriminate.
+      inv Hget. rewrite !FromList_cons in Hs. rewrite !FromList_cons.
+      eapply Union_Included.
+      + intros l' Hin. inv Hin. repeat eexists; eauto.
+      + eapply IHxs; eauto.
+        eapply Included_trans...
+  Qed.
+
+  Lemma well_formed_heap_eq S H1 H2 :
+    well_formed S H1 ->
+    closed S H1 -> 
+    S |- H1 ≡ H2 ->
+    well_formed S H2.
+  Proof.
+    intros Hwf Hcl Heq x v Hin Hget l Hin'.
+    rewrite <- Heq in Hget; eauto.
+    destruct (Hwf x v Hin Hget l Hin') as [l' Hget'].
+    rewrite -> Heq in Hget'; eauto. repeat eexists; eauto.
+    edestruct Hcl as [v' [Hget'' Hin'']]; eauto.
+    rewrite Hget in Hget''; inv Hget''; eauto.
+  Qed.    
+
+  Lemma heap_eq_dom {A} S (H1 H2 : heap A) S' :
+    S |- H1 ≡ H2 ->
+    S' \subset dom H1 ->
+    S' \subset S ->
+    S' \subset dom H2.
+  Proof.
+    intros Heq Hsub1 Hsub2 l Hin.
+    specialize (Hsub1 l Hin). destruct Hsub1 as [v Hget].
+    rewrite Heq in Hget; eauto.  eexists; eauto.
+  Qed.
+
+  Lemma alloc_In_dom {A} H1 (v :A) l H2 :
+    alloc v H1 = (l, H2) ->
+    l \in dom H2.
+  Proof.
+    intros. eexists. erewrite gas; eauto.
+  Qed.
+
+  (** Lemmas about [getlist] *)
+  Lemma getlist_In_val {A} (rho : M.t A) ys v vs :
+    getlist ys rho = Some vs ->
+    List.In v vs ->
+    exists x, List.In x ys /\ M.get x rho = Some v.
+  Proof.
+    revert v vs. induction ys; intros x vs Hget H.
+    - inv Hget. now inv H.
+    - simpl in *.
+      destruct (M.get a rho) eqn:Heq; try discriminate; eauto.
+      destruct (getlist ys rho) eqn:Heq'; try discriminate; eauto.
+      inv Hget. inv H; eauto.
+      edestruct IHys as [y [Hin Hget]]; eauto.
+  Qed.
+
+  Lemma heap_env_approx_Vfun S rho rho' rho1 rho2 H H' l l' f B :
+    M.get f rho = Some l ->
+    M.get f rho' = Some l' ->
+    (l, H) ≈ (l', H') ->
+    S |- (H, rho) ⩪ (H', rho') ->
+    f \in S ->
+    get l H = Some (Vfun rho1 B) ->
+    get l' H' = Some (Vfun rho2 B) ->
+    heap_env_approx (occurs_free_fundefs B) (H, rho1) (H', rho2).
+  Proof.
+    intros Hget1 Hget2 Heq Hheq Hin Hget1' Hget2' x1 l1 Hin' Hget.
+    edestruct Heq with (n := 1) as [Heq1 Heq2]. 
+    edestruct Heq1 as [v2 [Hget' Hv]]; eauto.
+    destruct v2; try contradiction.
+    destruct Hv as [HBeq Hlt]; subst. 
+    destruct (Hlt 0 x1) as [[l1' [l2' [Hgetl1 [Hgetl2 _]]]] | [Hn1 Hn2]]; eauto;
+    try congruence.
+    rewrite Hget in Hgetl1; inv Hgetl1; rewrite Hget' in  Hget2'; inv Hget2'.
+    eexists; split; eauto.
+    intros n.
+    edestruct Heq with (n := n + 1) as [Heqn1 Heqn2].
+    split.
+    - edestruct Heqn1 as [v2 [Hgetv Hv]]; eauto.
+      destruct v2; try contradiction. destruct Hv as [HBeq Hlt']; subst. 
+      destruct (Hlt' n x1) as [[l3' [l4' [Hgetl3 [Hgetl4 Hres]]]] | [Hn1 Hn2]]; eauto;
+      try congruence.
+      omega. rewrite Hgetv in Hget'; inv Hget'.
+      rewrite Hget in Hgetl3; inv Hgetl3.
+      rewrite Hgetl2 in Hgetl4; inv Hgetl4.
+      rewrite <- res_approx_fuel_eq. eassumption.
+    - edestruct Heqn2 as [v2 [Hgetv Hv]]; eauto.
+      destruct v2; try contradiction. destruct Hv as [HBeq Hlt']; subst. 
+      destruct (Hlt' n x1) as [[l3' [l4' [Hgetl3 [Hgetl4 Hres]]]] | [Hn1 Hn2]]; eauto;
+      try congruence.
+      omega. rewrite Hgetv in Hget1'; inv Hget1'.
+      rewrite Hget in Hgetl4; inv Hgetl4.
+      rewrite Hgetl2 in Hgetl3; inv Hgetl3.
+      rewrite <- res_approx_fuel_eq. eassumption.
+  Qed.
+
+  Corollary heap_env_equiv_Vfun S rho rho' rho1 rho2 H H' l l' f B :
+    M.get f rho = Some l ->
+    M.get f rho' = Some l' ->
+    (l, H) ≈ (l', H') ->
+    S |- (H, rho) ⩪ (H', rho') ->
+    f \in S ->
+    get l H = Some (Vfun rho1 B) ->
+    get l' H' = Some (Vfun rho2 B) ->
+    (occurs_free_fundefs B) |- (H, rho1) ⩪ (H', rho2).
+  Proof.
+    intros. split.
+    now eapply (heap_env_approx_Vfun _ rho rho' _ _ H H'); eauto.
+    now eapply (heap_env_approx_Vfun _ rho' rho _ _ H' H); eauto; symmetry.
+  Qed.
+
+  Lemma big_step_deterministic  H1 H2 rho1 rho2 e r1 c1 m1 r2 c2 m2 :
+    well_formed (reach' H1 (env_locs rho1 (occurs_free e))) H1 ->
+    well_formed (reach' H2 (env_locs rho2 (occurs_free e))) H2 ->
+    env_locs rho1 (occurs_free e) \subset dom H1 ->
+    env_locs rho2 (occurs_free e) \subset dom H2 ->
+    big_step H1 rho1 e r1 c1 m1 -> (* D1 *)
+    big_step H2 rho2 e r2 c2 m2 -> (* D2 *)
+    (occurs_free e) |- (H1, rho1) ⩪ (H2, rho2) ->
+    c1 = c2 /\ r1 ≈ r2.
+  Proof with now eauto with Ensembles_DB.
+     (* Lexicographic induction on the size of the first derivation and the size of the second derivation *)
+     intros Hwf1 Hwf2 Hwfe1 Hwfe2 Hbs1 Hbs2. remember (size_big_step Hbs1) as n.
+     revert H1 H2 rho1 rho2 e r1 c1 m1 r2 c2 m2 Hwf1 Hwf2 Hwfe1 Hwfe2 Hbs1 Heqn Hbs2.
+     induction n as [n IH1] using lt_wf_rec1.
+     intros H1 H2 rho1 rho2 e r1 c1 m1 r2 c2 m2 Hwf1 Hwf2 Hwfe1 Hwfe2 Hbs1 Heqn Hbs2.
+     subst.
+     remember (size_big_step Hbs2) as m.
+     revert H1 H2 rho1 rho2 e r1 c1 m1 r2 c2 m2 Hwf1 Hwf2 Hwfe1 Hwfe2 Hbs1 Hbs2 Heqm IH1.
+     induction m as [m IH2] using lt_wf_rec1.  
+     intros H1 H2 rho1 rho2 e r1 c1 m1 r2 c2 m2 Hwf1 Hwf2 Hwfe1 Hwfe2 Hbs1 Hbs2 Heqm IH1 Heq.
+     destruct Hbs1; simpl in *. 
+     - (* D1 : Eval_case *)
+       subst m. remember (Econstr x t ys e) as e'. destruct Hbs2; inv Heqe'; simpl in *.
+       + (* D2 : Eval_case *)
+         eapply IH1 with (Hbs1 := Hbs1); [ | | | | | reflexivity | |]. 
+         * omega.
+         * eapply well_formed_antimon. eapply reach'_set_monotonic.
+           eapply env_locs_monotonic. now apply occurs_free_Econstr_Included.
+           eapply well_formed_reach_alloc with (H := H); eauto.
+           eapply Included_trans; [| now apply reach'_extensive ].
+           simpl. eapply FromList_env_locs; eauto. normalize_occurs_free...
+         * eapply well_formed_antimon. eapply reach'_set_monotonic.
+           eapply env_locs_monotonic. now apply occurs_free_Econstr_Included.
+           eapply well_formed_reach_alloc with (H := H0); eauto.
+           eapply Included_trans; [| now apply reach'_extensive ].
+           simpl. eapply FromList_env_locs; eauto. normalize_occurs_free...
+         * eapply Included_trans.
+           eapply env_locs_monotonic. now apply occurs_free_Econstr_Included.
+           eapply Included_trans. eapply env_locs_set_Inlcuded.
+           eapply Union_Included. eapply Singleton_Included.
+           now eapply alloc_In_dom; eauto.
+           eapply Included_trans. eassumption.
+           eapply dom_subheap. now eapply alloc_subheap; eauto.
+         * eapply Included_trans.
+           eapply env_locs_monotonic. now apply occurs_free_Econstr_Included.
+           eapply Included_trans. eapply env_locs_set_Inlcuded.
+           eapply Union_Included. eapply Singleton_Included.
+           now eapply alloc_In_dom; eauto.
+           eapply Included_trans. eassumption.
+           eapply dom_subheap. now eapply alloc_subheap; eauto.
+         * now apply Hbs2.
+         * eapply (heap_env_equiv_set_alloc_Vconstr _ _ _ H H0); eauto. 
+           eapply reach'_closed. eassumption. eassumption.
+           eapply reach'_closed. eassumption. eassumption.
+           eapply Included_trans; [| now apply reach'_extensive ].
+           eapply env_locs_monotonic. normalize_occurs_free...
+           eapply Included_trans; [| now apply reach'_extensive ].
+           eapply env_locs_monotonic. normalize_occurs_free...
+           eapply Included_trans; [| now apply reach'_extensive ].
+           eapply FromList_env_locs; eauto. normalize_occurs_free...
+           eapply Included_trans; [| now apply reach'_extensive ].
+           eapply FromList_env_locs; eauto. normalize_occurs_free...
+           eapply heap_env_equiv_antimon. eassumption.
+           eapply Setminus_Included_Included_Union. now eapply occurs_free_Econstr_Included.
+           eapply Forall2_symm_strong; [| eapply heap_env_equiv_getlist_Forall2 ]. 
+           intros. now symmetry. now split; eapply Heq.
+           rewrite occurs_free_Econstr... eassumption. eassumption.
+       + (* D2 : Eval_GC *)
+         assert (Hex : exists  (Hbs1' : big_step H rho (Econstr x t ys e) r c m0), size_big_step Hbs1' = S (size_big_step Hbs1)).
+         { exists (Eval_constr H H' rho (M.set x l rho)  x t ys e ls l r c m0 e0 e1 Hbs1).
+           reflexivity. }
+         destruct Hex as [Hbs1' Hsize]. 
+         eapply IH2 with (Hbs2 := Hbs2) (Hbs1 := Hbs1'); [ | | | | | reflexivity | | ]; try eassumption.
+         * omega.
+         * rewrite <- reach'_heap_eq; eauto. eapply well_formed_heap_eq.
+           eassumption. now eapply reach'_closed; eauto. eassumption.
+         * eapply heap_eq_dom; eauto. now apply reach'_extensive.
+         * intros. subst. eapply IH1 with (Hbs1 := Hbs0); [| | | | | reflexivity | |]; try eassumption.
+           omega.
+         * edestruct Equivalence_heap_env_equiv. eapply Equivalence_Transitive; eauto.
+           eapply reach_heap_env_equiv. eapply reach'_heap_eq. eassumption. eassumption.
+     - subst m. remember (Eproj x t n y e) as e'. destruct Hbs2; inv Heqe'; simpl in *.
+       + eapply IH1 with (Hbs1 := Hbs1); [ | | | | | reflexivity | |]; try eassumption.   
+         * omega.
+         * eapply well_formed_antimon. eapply reach'_set_monotonic.
+           eapply Included_trans.
+           eapply env_locs_monotonic. now apply occurs_free_Eproj_Included.
+           eapply env_locs_set_Inlcuded.
+           rewrite <-reach_spec. eassumption. now eauto with Ensembles_DB.
+           eapply Union_Included.
+           eapply Singleton_Included. eexists 1.
+           split. now constructor. eexists l. eexists.
+           repeat split; eauto; simpl. now eexists; split; eauto.
+           now eapply nthN_In; eauto.
+           now apply reach'_extensive.
+         * eapply well_formed_antimon. eapply reach'_set_monotonic.
+           eapply Included_trans.
+           eapply env_locs_monotonic. now apply occurs_free_Eproj_Included.
+           eapply env_locs_set_Inlcuded.
+           rewrite <-reach_spec. eassumption. now eauto with Ensembles_DB.
+           eapply Union_Included.
+           eapply Singleton_Included. eexists 1. split.
+           now constructor.
+           eexists l0. eexists. repeat split; eauto; simpl.
+           now eexists; split; eauto.
+           now eapply nthN_In; eauto.
+           now apply reach'_extensive.
+         * eapply Included_trans.
+           eapply env_locs_monotonic. now apply occurs_free_Eproj_Included.
+           eapply Included_trans. eapply env_locs_set_Inlcuded.
+           eapply Union_Included; [| eassumption ].
+           eapply Singleton_Included. eapply reachable_in_dom; eauto.
+           eexists 1. split.
+           now constructor.
+           eexists l. eexists. repeat split; eauto; simpl.
+           now eexists; split; eauto. now eapply nthN_In; eauto.
+         * eapply Included_trans.
+           eapply env_locs_monotonic. now apply occurs_free_Eproj_Included.
+           eapply Included_trans. eapply env_locs_set_Inlcuded.
+           eapply Union_Included; [| eassumption ].
+           eapply Singleton_Included. eapply reachable_in_dom; eauto.
+           eexists 1. split.
+           now constructor.
+           eexists l0. eexists. repeat split; eauto; simpl.
+           now eexists; split; eauto. now eapply nthN_In; eauto.
+         * eapply heap_env_equiv_set.
+           eapply heap_env_equiv_antimon. eassumption.
+           eapply Setminus_Included_Included_Union. now eapply occurs_free_Eproj_Included.
+           eapply Heq in e0. destruct e0 as [l2' [Hget' Heq']]. rewrite e4  in Hget'. inv Hget'.
+           intros n'; split.
+           { eapply Heq' with (n := S n') in e1.
+             destruct e1 as [v2 [Hgetv2 Hequiv]]. rewrite e5 in Hgetv2. inv Hgetv2.
+             edestruct (@Forall2_nthN loc loc) as [l1' [Hnth Heql1']]; [ eapply Hequiv with (i := n')| | ]; eauto.
+             rewrite e6 in Hnth; inv Hnth. now rewrite <- res_approx_fuel_eq. }
+           { eapply Heq' with (n := S n') in e5.
+             destruct e5 as [v2 [Hgetv2 Hequiv]]. rewrite e1 in Hgetv2. inv Hgetv2.
+             edestruct (@Forall2_nthN loc loc) as [l1' [Hnth Heql1']]; [ eapply Hequiv with (i := n')| | ]; eauto.
+             rewrite e2 in Hnth; inv Hnth. now rewrite <- res_approx_fuel_eq. }
+           now eauto.
+       + assert (Hex : exists  (Hbs1' : big_step H rho (Eproj x t n y e) r c m0), size_big_step Hbs1' = S (size_big_step Hbs1)).
+         { exists (Eval_proj H rho x t n y e l l' ls r c m0 e0 e1 e2 Hbs1).
+           reflexivity. }
+        destruct Hex as [Hbs1' Hsize].
+        eapply IH2 with (Hbs2 := Hbs2) (Hbs1 := Hbs1'); [ | | | | | reflexivity | | ]; try eassumption.
+         * omega.
+         * rewrite <- reach'_heap_eq; eauto. eapply well_formed_heap_eq.
+           eassumption. now eapply reach'_closed; eauto. eassumption.
+         * eapply heap_eq_dom; eauto. now apply reach'_extensive.
+         * intros. subst. eapply IH1 with (Hbs1 := Hbs0); [| | | | | reflexivity | |]; try eassumption.
+           omega.
+         * edestruct Equivalence_heap_env_equiv. eapply Equivalence_Transitive; eauto.
+           eapply reach_heap_env_equiv. eapply reach'_heap_eq. eassumption. eassumption.
+     - subst m. remember (Ecase y cl) as e'. destruct Hbs2; inv Heqe'; simpl in *.
+       + eapply Heq in e0. edestruct e0 as [l' [Hget Heql']]. rewrite e4 in Hget; inv Hget.
+         eapply Heql' with (n := 0) in e1. destruct e1 as [v' [Hget' Heql'']]. rewrite e5 in Hget'. inv Hget'.
+         eapply Heql' with (n := 0) in e5.  inv Heql''. rewrite e2 in e6; inv e6.
+         eapply IH1 with (Hbs1 := Hbs1); [ | | | | | reflexivity | | ]; try eassumption; eauto.   
+         * eapply well_formed_antimon; [| eassumption ].
+           eapply reach'_set_monotonic. eapply env_locs_monotonic.
+           rewrite occurs_free_Ecase_Included. reflexivity.
+           eapply cps_util.findtag_In. eassumption.
+         * eapply well_formed_antimon; [| eassumption ].
+           eapply reach'_set_monotonic. eapply env_locs_monotonic.
+           rewrite occurs_free_Ecase_Included. reflexivity.
+           eapply cps_util.findtag_In. eassumption.
+         * eapply Included_trans; [| eassumption ].
+           eapply env_locs_monotonic.
+           rewrite occurs_free_Ecase_Included. reflexivity.
+           eapply cps_util.findtag_In. eassumption.
+         * eapply Included_trans; [| eassumption ].
+           eapply env_locs_monotonic.
+           rewrite occurs_free_Ecase_Included. reflexivity.
+           eapply cps_util.findtag_In. eassumption.
+         * eapply heap_env_equiv_antimon.
+           eassumption.
+           rewrite occurs_free_Ecase_Included. reflexivity.
+           eapply cps_util.findtag_In. eassumption.
+         * eauto.
+       + assert (Hex : exists  (Hbs1' : big_step H rho (Ecase y cl) r c m0), size_big_step Hbs1' = S (size_big_step Hbs1)).
+         { exists (Eval_case H rho y cl l t ls e r c m0 e0 e1 e2 Hbs1). reflexivity. }
+         destruct Hex as [Hbs1' Hsize].
+         eapply IH2 with (Hbs2 := Hbs2) (Hbs1 := Hbs1'); [ | | | | | reflexivity | | ]; try eassumption.
+         * omega.
+         * rewrite <- reach'_heap_eq; eauto. eapply well_formed_heap_eq.
+           eassumption. now eapply reach'_closed; eauto. eassumption.
+         * eapply heap_eq_dom; eauto. now apply reach'_extensive.
+         * intros. subst. eapply IH1 with (Hbs1 := Hbs0); [| | | | | reflexivity | |]; try eassumption.
+           omega.
+         * edestruct Equivalence_heap_env_equiv. eapply Equivalence_Transitive; eauto.
+           eapply reach_heap_env_equiv. eapply reach'_heap_eq. eassumption. eassumption.
+     - subst m. remember (Efun B e) as e'. destruct Hbs2; inv Heqe'; simpl in *.
+       + eapply IH1 with (Hbs1 := Hbs1); [| | | | | reflexivity | eassumption |].
+         * omega.
+         * eapply well_formed_antimon. eapply reach'_set_monotonic.
+           eapply env_locs_monotonic. now apply occurs_free_Efun_Included.
+           eapply well_formed_reach_alloc_def_funs; eauto.
+           simpl. eapply Included_trans; [| now eapply reach'_extensive ].
+           eapply env_locs_monotonic. normalize_occurs_free...
+         * eapply well_formed_antimon. eapply reach'_set_monotonic.
+           eapply env_locs_monotonic. now apply occurs_free_Efun_Included.
+           eapply well_formed_reach_alloc_def_funs; eauto.
+           simpl. eapply Included_trans; [| now eapply reach'_extensive ].
+           eapply env_locs_monotonic. normalize_occurs_free...
+         * eapply Included_trans.
+           eapply env_locs_monotonic. now apply occurs_free_Efun_Included.
+           eapply Included_trans. eapply env_locs_def_funs_Included.
+           eapply Union_Included.
+           eapply Included_trans. eassumption.
+           eapply dom_subheap. now eapply alloc_subheap; eauto.
+           eapply Singleton_Included.
+           now eapply alloc_In_dom; eauto.
+         * eapply Included_trans.
+           eapply env_locs_monotonic. now apply occurs_free_Efun_Included.
+           eapply Included_trans. eapply env_locs_def_funs_Included.
+           eapply Union_Included.
+           eapply Included_trans. eassumption.
+           eapply dom_subheap. now eapply alloc_subheap; eauto.
+           eapply Singleton_Included.
+           now eapply alloc_In_dom; eauto.
+         * eapply heap_env_equiv_antimon; [| now apply occurs_free_Efun_Included ].
+           eapply (heap_env_equiv_def_funs_alloc _ _ _ H H0).
+           now eapply reach'_closed; eauto.
+           now eapply reach'_closed; eauto.
+           eapply Included_trans; [| now apply reach'_extensive ].
+           eapply env_locs_monotonic...
+           eapply Included_trans; [| now apply reach'_extensive ].
+           eapply env_locs_monotonic...
+           rewrite Setminus_Union_distr, Setminus_Same_set_Empty_set, Union_Empty_set_neut_r.
+           rewrite Setminus_Disjoint. normalize_occurs_free...
+           normalize_occurs_free.
+           eapply Union_Disjoint_l.
+           constructor. intros x Hc. inv Hc; eapply fun_names_not_free_in_fundefs; eauto.
+           eapply Disjoint_Setminus_l...
+           rewrite Setminus_Union_distr, Setminus_Same_set_Empty_set, Union_Empty_set_neut_r.
+           eapply heap_env_equiv_antimon; [ eassumption | ]...
+           eassumption. eassumption.
+       + assert (Hex : exists  (Hbs1' : big_step H rho (Efun B e) r c m0), size_big_step Hbs1' = S (size_big_step Hbs1)).
+         { exists (Eval_fun H H' rho B l e r c m0 e0 Hbs1).
+           reflexivity. }
+         destruct Hex as [Hbs1' Hsize].
+         eapply IH2 with (Hbs2 := Hbs2) (Hbs1 := Hbs1'); [| | |  | | reflexivity | | ]; try eassumption.
+         * omega.
+         * rewrite <- reach'_heap_eq; eauto. eapply well_formed_heap_eq.
+           eassumption. now eapply reach'_closed; eauto. eassumption.
+         * eapply heap_eq_dom; eauto. now apply reach'_extensive.
+         * intros. subst. eapply IH1 with (Hbs1 := Hbs0); [| | | | | reflexivity | |]; try eassumption.
+           omega.
+         * edestruct Equivalence_heap_env_equiv. eapply Equivalence_Transitive; eauto.
+           eapply reach_heap_env_equiv. eapply reach'_heap_eq. eassumption. eassumption.
+     - subst m. remember (Eapp f t ys) as e'. destruct Hbs2; inv Heqe'; simpl in *.
+       + assert (c  = c0 /\ r ≈ r0).
+         { assert (Hgetf' := e6). assert (Hgetl' := e7).
+           eapply Heq in e6. destruct e6 as [l' [Hget Hequiv]].
+           rewrite Hget in e0; inv e0. eapply Hequiv with (n := 1) in e7.
+           destruct e7 as [v2 [Hget2 Heq2]]. rewrite Hget2 in e1. inv e1.
+           inv Heq2. rewrite e9 in e3; inv e3.
+           assert (Hreach1 : reach' H (env_locs rho' (occurs_free_fundefs B)) \subset
+                             reach' H (env_locs rho (occurs_free (Eapp f t ys)))).
+           { rewrite (reach_unfold H (env_locs rho _) ).
+             eapply Included_Union_preserv_r. eapply reach'_set_monotonic.
+             intros l1 H1. do 2 eexists. repeat split; eauto.
+             eexists f. now split; eauto. }
+           assert (Hreach2 : reach' H0 (env_locs rho'0 (occurs_free_fundefs B)) \subset
+                             reach' H0 (env_locs rho0 (occurs_free (Eapp f t ys)))).
+           { rewrite (reach_unfold H0 (env_locs rho0 _) ).
+             eapply Included_Union_preserv_r. eapply reach'_set_monotonic.
+             intros l1 [x [Hin1 Hget1]].
+             repeat eexists; eauto. repeat eexists; eauto. }
+           eapply IH1 with (Hbs1 := Hbs1); [| | | | | reflexivity | eassumption |].         
+           - omega.
+           - eapply well_formed_antimon; [| eassumption ].
+             eapply Included_trans. eapply reach'_set_monotonic.
+             eapply env_locs_monotonic. eapply occurs_free_in_fun.
+             eapply find_def_correct. eassumption. rewrite Union_commut.
+             eapply Included_trans. eapply reach'_set_monotonic.
+             eapply env_locs_set_list_Included; eauto.
+             rewrite (Union_commut (name_in_fundefs B) (occurs_free_fundefs B)).
+             eapply Included_trans. eapply reach'_set_monotonic. eapply Included_Union_compat.
+             eapply env_locs_def_funs_Included. reflexivity.
+             rewrite !reach'_Union. eapply Union_Included; [ eapply Union_Included |].
+             + eassumption.
+             + eapply reach'_set_monotonic.
+               intros l1 H1. inv H1. do 2 eexists. repeat split; eauto.
+               eassumption. 
+             + eapply reach'_set_monotonic.
+               intros l1 H1. edestruct (@getlist_In_val loc) as [y [Hin' Hget']]; [| eassumption |]; eauto.
+               exists y; split; eauto.
+           - eapply well_formed_antimon; [| eassumption ].
+             eapply Included_trans. eapply reach'_set_monotonic.
+             eapply env_locs_monotonic. eapply occurs_free_in_fun.
+             eapply find_def_correct. eassumption. rewrite Union_commut.
+             eapply Included_trans. eapply reach'_set_monotonic.
+             eapply env_locs_set_list_Included; eauto.
+             rewrite (Union_commut (name_in_fundefs B) (occurs_free_fundefs B)).
+             eapply Included_trans. eapply reach'_set_monotonic. eapply Included_Union_compat.
+             eapply env_locs_def_funs_Included. reflexivity.
+             rewrite !reach'_Union. eapply Union_Included; [ eapply Union_Included |].
+             + eassumption.
+             + eapply reach'_set_monotonic.
+               intros l1 H1. inv H1. do 2 eexists. repeat split; eauto.
+               eassumption. 
+             + eapply reach'_set_monotonic.
+               intros l1 H1. edestruct (@getlist_In_val loc) as [y [Hin' Hget']]; [| eassumption |]; eauto.
+               exists y; split; eauto.
+           - eapply Included_trans. eapply env_locs_monotonic. eapply occurs_free_in_fun.
+             eapply find_def_correct. eassumption. rewrite Union_commut.
+             eapply Included_trans. eapply env_locs_set_list_Included; eauto.
+             rewrite (Union_commut (name_in_fundefs B) (occurs_free_fundefs B)).
+             eapply Included_trans. eapply Included_Union_compat.
+             eapply env_locs_def_funs_Included. reflexivity.
+             eapply Union_Included; [ eapply Union_Included |].
+             eapply Included_trans; [| now eapply reachable_in_dom; eauto ].
+             eapply Included_trans. now apply reach'_extensive. eassumption.
+             eapply Singleton_Included. now eexists; eauto.
+             eapply Included_trans; [| eassumption ].
+             eapply FromList_env_locs; eauto. normalize_occurs_free...
+           - eapply Included_trans. eapply env_locs_monotonic. eapply occurs_free_in_fun.
+             eapply find_def_correct. eassumption. rewrite Union_commut.
+             eapply Included_trans. eapply env_locs_set_list_Included; eauto.
+             rewrite (Union_commut (name_in_fundefs B) (occurs_free_fundefs B)).
+             eapply Included_trans. eapply Included_Union_compat.
+             eapply env_locs_def_funs_Included. reflexivity.
+             eapply Union_Included; [ eapply Union_Included |].
+             eapply Included_trans; [| now eapply reachable_in_dom; eauto ].
+             eapply Included_trans. now apply reach'_extensive. eassumption.
+             eapply Singleton_Included. now eexists; eauto.
+             eapply Included_trans; [| eassumption ].
+             eapply FromList_env_locs; eauto. normalize_occurs_free...
+           - eapply heap_env_equiv_setlist; eauto.
+             eapply heap_env_equiv_def_funs; eauto.
+             eapply heap_env_equiv_antimon.
+             eapply (heap_env_equiv_Vfun _ rho rho0); eauto. symmetry. eassumption.
+             rewrite Setminus_Union. apply Setminus_Included_Included_Union.
+             eapply Included_trans. eapply occurs_free_in_fun.
+             eapply find_def_correct; eauto. now eauto with Ensembles_DB.
+             symmetry. eassumption. 
+             eapply heap_env_equiv_getlist_Forall2; eauto.
+             normalize_occurs_free...
+           - eauto. }
+         firstorder.
+       + assert (Hex : exists  (Hbs1' : big_step H rho (Eapp f t ys) r (c+1) m0), size_big_step Hbs1' = S (size_big_step Hbs1)).
+         { exists (Eval_app H rho rho' rho'' B f t xs e l ls ys r c m0 e0 e1 e2 e3 e4 Hbs1).
+           reflexivity. }
+         destruct Hex as [Hbs1' Hsize].
+         eapply IH2 with (Hbs2 := Hbs2) (Hbs1 := Hbs1'); [| | | | | reflexivity | | ]; try eassumption.
+         * omega.
+         * rewrite <- reach'_heap_eq; eauto. eapply well_formed_heap_eq.
+           eassumption. now eapply reach'_closed; eauto. eassumption.
+         * eapply heap_eq_dom; eauto. now apply reach'_extensive.
+         * intros. subst. eapply IH1 with (Hbs1 := Hbs0); [| | | | | reflexivity | |]; try eassumption.
+           omega.
+         * edestruct Equivalence_heap_env_equiv. eapply Equivalence_Transitive; eauto.
+           eapply reach_heap_env_equiv. eapply reach'_heap_eq. eassumption. eassumption.
+     - subst m. remember (Ehalt x) as e'. destruct Hbs2; inv Heqe'; simpl in *.
+       + split; eauto.
+         eapply Heq in e0. destruct e0 as [l' [Hget Hequiv]].
+         rewrite e in Hget; inv Hget. symmetry. eassumption.
+         now eauto.
+       + assert (Hex : exists  (Hbs1' : big_step H rho (Ehalt x) (l, H) 0 m0), size_big_step Hbs1' = 0).
+         { exists (Eval_halt H rho x l m0 e s). eauto. }
+         destruct Hex as [Hbs1' Hsize].
+         eapply IH2 with (Hbs2 := Hbs2) (Hbs1 := Hbs1'); [| | | | | reflexivity | | ]; try eassumption.
+         * omega.
+         * rewrite <- reach'_heap_eq; eauto. eapply well_formed_heap_eq.
+           eassumption. now eapply reach'_closed; eauto. eassumption.
+         * eapply heap_eq_dom; eauto. now apply reach'_extensive.
+         * intros. subst. eapply IH1 with (Hbs1 := Hbs1); [| | | | | reflexivity | |]; try eassumption.
+           omega. 
+         * edestruct Equivalence_heap_env_equiv. eapply Equivalence_Transitive; eauto.
+           eapply reach_heap_env_equiv. eapply reach'_heap_eq. eassumption. eassumption.
+     - eapply IH1 with (Hbs1 := Hbs1); [| | | | | reflexivity | eassumption |].
+       + omega.
+       + rewrite <- reach'_heap_eq; eauto. eapply well_formed_heap_eq.
+         eassumption. now eapply reach'_closed; eauto. eassumption.
+       + eassumption.
+       + eapply heap_eq_dom; try eassumption. now apply reach'_extensive.
+       + eassumption.
+       + edestruct Equivalence_heap_env_equiv. eapply Equivalence_Transitive; try eassumption.
+         symmetry. eapply reach_heap_env_equiv. eapply reach'_heap_eq. eassumption.
+         eassumption.
+  Qed.  
+
 
 End Sem.
